src/fi/abo/it/actortool/Ast.scala
@@ -130,12 +130,18 @@ object Count {
   def reset = {i = -1}
 }
 
+object ActionClass extends Enumeration {
+  val Normal, Primary, Error, Recovery = Value
+}
+
 sealed case class Action(
-    private val label: Option[String], val init: Boolean, 
+    val label: Option[String], val aClass: ActionClass.Value, val init: Boolean, 
     val inputPattern: List[InputPattern], val outputPattern: List[OutputPattern],
     val guard: Option[Expr], 
     val requires: List[Expr], val ensures: List[Expr], variables: List[Declaration],
     val body: Option[List[Stmt]]) extends Member {
+  
+  
 
  //var transitions: List[(String,String)] = Nil
   
