ft_tests/Add.bpl
@@ -53,7 +53,7 @@ const unique Net#add: Actor;
 const unique Net#a: Chan (int);
 const unique Net#b: Chan (int);
 const unique Net#c: Chan (int);
-procedure Net#anon$2#entry#2()
+procedure Net#anon$1#entry#2()
   modifies C, R, M, St, SqnCh, SqnAct;
 {
   assume SqnAct[Net#add] == 0;
@@ -65,8 +65,11 @@ procedure Net#anon$2#entry#2()
   assume C[Net#b] == 0;
   assume R[Net#c] == 0;
   assume C[Net#c] == 0;
-  assume (forall idx$: int :: 
-    (0 <= idx$) && (idx$ < L[Net#a]) ==> (0 <= M[Net#a][idx$]) && (0 <= M[Net#b][idx$])
+  assume (forall i: int :: 
+    (0 <= i) && (i < L[Net#a]) ==> (0 <= M[Net#a][i])
+  );
+  assume (forall i: int :: 
+    (0 <= i) && (i < L[Net#b]) ==> (0 <= M[Net#b][i])
   );
   assume 0 <= R[Net#a];
   assume 0 <= C[Net#a];
@@ -77,29 +80,32 @@ procedure Net#anon$2#entry#2()
   assume 0 <= R[Net#c];
   assume 0 <= C[Net#c];
   assume R[Net#c] == 0;
-  assert {:msg "  Channel invariant might not hold on action entry (#9)"} (forall idx$: int :: 
-    (0 <= idx$) && (idx$ < L[Net#a]) ==> (0 <= M[Net#a][idx$]) && (0 <= M[Net#b][idx$])
+  assert {:msg "  Channel invariant might not hold on action entry (#9)"} (forall i: int :: 
+    (0 <= i) && (i < L[Net#a]) ==> (0 <= M[Net#a][i])
   );
-  assert {:msg "  Channel invariant might not hold on action entry (#10)"} R[Net#a] == (R[Net#c] + C[Net#c]);
-  assert {:msg "  Channel invariant might not hold on action entry (#11)"} R[Net#b] == (R[Net#c] + C[Net#c]);
-  assert {:msg "  Channel invariant might not hold on action entry (#12)"} (forall idx$: int :: 
+  assert {:msg "  Channel invariant might not hold on action entry (#10)"} (forall i: int :: 
+    (0 <= i) && (i < L[Net#b]) ==> (0 <= M[Net#b][i])
+  );
+  assert {:msg "  Channel invariant might not hold on action entry (#11)"} R[Net#a] == (R[Net#c] + C[Net#c]);
+  assert {:msg "  Channel invariant might not hold on action entry (#12)"} R[Net#b] == (R[Net#c] + C[Net#c]);
+  assert {:msg "  Channel invariant might not hold on action entry (#13)"} (forall idx$: int :: 
     (0 <= idx$) && (idx$ < (R[Net#c] + C[Net#c])) ==> (M[Net#c][idx$] == (M[Net#a][idx$] + M[Net#b][idx$]))
   );
-  assert {:msg "  Channel invariant might not hold on action entry (#13)"} (forall idx$: int :: 
+  assert {:msg "  Channel invariant might not hold on action entry (#14)"} (forall idx$: int :: 
     (0 <= idx$) && (idx$ < (R[Net#a] + C[Net#a])) ==> (SqnCh[Net#a][idx$] == idx$)
   );
-  assert {:msg "  Channel invariant might not hold on action entry (#14)"} (forall idx$: int :: 
+  assert {:msg "  Channel invariant might not hold on action entry (#15)"} (forall idx$: int :: 
     (0 <= idx$) && (idx$ < (R[Net#b] + C[Net#b])) ==> (SqnCh[Net#b][idx$] == idx$)
   );
-  assert {:msg "  16.3: Channel invariant might not hold on action entry (#15)"} SqnAct[Net#add] == R[Net#a];
-  assert {:msg "  17.3: Channel invariant might not hold on action entry (#16)"} (forall i: int :: 
+  assert {:msg "  17.3: Channel invariant might not hold on action entry (#16)"} SqnAct[Net#add] == R[Net#a];
+  assert {:msg "  18.3: Channel invariant might not hold on action entry (#17)"} (forall i: int :: 
     (0 <= i) && (i < (R[Net#a] + C[Net#a])) ==> (SqnCh[Net#a][i] == SqnCh[Net#b][i])
   );
-  assert {:msg "  18.3: Channel invariant might not hold on action entry (#17)"} (forall i: int :: 
+  assert {:msg "  19.3: Channel invariant might not hold on action entry (#18)"} (forall i: int :: 
     (0 <= i) && (i < R[Net#a]) ==> (SqnCh[Net#a][i] == SqnCh[Net#c][i])
   );
 }
-procedure Net#anon$2#Add#anon$0#3()
+procedure Net#anon$1#Add#anon$0#3()
   modifies C, R, M, St, SqnCh, SqnAct;
 {
   var St#next: State;
@@ -116,8 +122,11 @@ procedure Net#anon$2#Add#anon$0#3()
   assume 0 <= R[Net#c];
   assume 0 <= C[Net#c];
   assume R[Net#c] == 0;
-  assume (forall idx$: int :: 
-    (0 <= idx$) && (idx$ < L[Net#a]) ==> (0 <= M[Net#a][idx$]) && (0 <= M[Net#b][idx$])
+  assume (forall i: int :: 
+    (0 <= i) && (i < L[Net#a]) ==> (0 <= M[Net#a][i])
+  );
+  assume (forall i: int :: 
+    (0 <= i) && (i < L[Net#b]) ==> (0 <= M[Net#b][i])
   );
   assume R[Net#a] == (R[Net#c] + C[Net#c]);
   assume R[Net#b] == (R[Net#c] + C[Net#c]);
@@ -139,7 +148,7 @@ procedure Net#anon$2#Add#anon$0#3()
   );
   assume true;
   assume (1 <= C[Net#a]) && (1 <= C[Net#b]);
-  assert {:msg "  4.14: Precondition might not hold for instance at 21.5"} SqnCh[Net#a][R[Net#a] - 0] == SqnCh[Net#b][R[Net#b] - 0];
+  assert {:msg "  4.14: Precondition might not hold for instance at 22.5"} SqnCh[Net#a][R[Net#a] - 0] == SqnCh[Net#b][R[Net#b] - 0];
   in1#i := M[Net#a][R[Net#a]];
   R[Net#a] := R[Net#a] + 1;
   C[Net#a] := C[Net#a] - 1;
@@ -159,29 +168,32 @@ procedure Net#anon$2#Add#anon$0#3()
   assume 0 <= R[Net#c];
   assume 0 <= C[Net#c];
   assume R[Net#c] == 0;
-  assert {:msg "  Action at 3.3 ('anon$0') for actor instance 'add' might not preserve the channel invariant (#27)"} (forall idx$: int :: 
-    (0 <= idx$) && (idx$ < L[Net#a]) ==> (0 <= M[Net#a][idx$]) && (0 <= M[Net#b][idx$])
+  assert {:msg "  Action at 3.3 ('anon$0') for actor instance 'add' might not preserve the channel invariant (#28)"} (forall i: int :: 
+    (0 <= i) && (i < L[Net#a]) ==> (0 <= M[Net#a][i])
   );
-  assert {:msg "  Action at 3.3 ('anon$0') for actor instance 'add' might not preserve the channel invariant (#28)"} R[Net#a] == (R[Net#c] + C[Net#c]);
-  assert {:msg "  Action at 3.3 ('anon$0') for actor instance 'add' might not preserve the channel invariant (#29)"} R[Net#b] == (R[Net#c] + C[Net#c]);
-  assert {:msg "  Action at 3.3 ('anon$0') for actor instance 'add' might not preserve the channel invariant (#30)"} (forall idx$: int :: 
+  assert {:msg "  Action at 3.3 ('anon$0') for actor instance 'add' might not preserve the channel invariant (#29)"} (forall i: int :: 
+    (0 <= i) && (i < L[Net#b]) ==> (0 <= M[Net#b][i])
+  );
+  assert {:msg "  Action at 3.3 ('anon$0') for actor instance 'add' might not preserve the channel invariant (#30)"} R[Net#a] == (R[Net#c] + C[Net#c]);
+  assert {:msg "  Action at 3.3 ('anon$0') for actor instance 'add' might not preserve the channel invariant (#31)"} R[Net#b] == (R[Net#c] + C[Net#c]);
+  assert {:msg "  Action at 3.3 ('anon$0') for actor instance 'add' might not preserve the channel invariant (#32)"} (forall idx$: int :: 
     (0 <= idx$) && (idx$ < (R[Net#c] + C[Net#c])) ==> (M[Net#c][idx$] == (M[Net#a][idx$] + M[Net#b][idx$]))
   );
-  assert {:msg "  Action at 3.3 ('anon$0') for actor instance 'add' might not preserve the channel invariant (#31)"} (forall idx$: int :: 
+  assert {:msg "  Action at 3.3 ('anon$0') for actor instance 'add' might not preserve the channel invariant (#33)"} (forall idx$: int :: 
     (0 <= idx$) && (idx$ < (R[Net#a] + C[Net#a])) ==> (SqnCh[Net#a][idx$] == idx$)
   );
-  assert {:msg "  Action at 3.3 ('anon$0') for actor instance 'add' might not preserve the channel invariant (#32)"} (forall idx$: int :: 
+  assert {:msg "  Action at 3.3 ('anon$0') for actor instance 'add' might not preserve the channel invariant (#34)"} (forall idx$: int :: 
     (0 <= idx$) && (idx$ < (R[Net#b] + C[Net#b])) ==> (SqnCh[Net#b][idx$] == idx$)
   );
-  assert {:msg "  16.3: Action at 3.3 ('anon$0') for actor instance 'add' might not preserve the channel invariant (#33)"} SqnAct[Net#add] == R[Net#a];
-  assert {:msg "  17.3: Action at 3.3 ('anon$0') for actor instance 'add' might not preserve the channel invariant (#34)"} (forall i: int :: 
+  assert {:msg "  17.3: Action at 3.3 ('anon$0') for actor instance 'add' might not preserve the channel invariant (#35)"} SqnAct[Net#add] == R[Net#a];
+  assert {:msg "  18.3: Action at 3.3 ('anon$0') for actor instance 'add' might not preserve the channel invariant (#36)"} (forall i: int :: 
     (0 <= i) && (i < (R[Net#a] + C[Net#a])) ==> (SqnCh[Net#a][i] == SqnCh[Net#b][i])
   );
-  assert {:msg "  18.3: Action at 3.3 ('anon$0') for actor instance 'add' might not preserve the channel invariant (#35)"} (forall i: int :: 
+  assert {:msg "  19.3: Action at 3.3 ('anon$0') for actor instance 'add' might not preserve the channel invariant (#37)"} (forall i: int :: 
     (0 <= i) && (i < R[Net#a]) ==> (SqnCh[Net#a][i] == SqnCh[Net#c][i])
   );
 }
-procedure Net#anon$2#exit#4()
+procedure Net#anon$1#exit#4()
   modifies C, R, M, St, SqnCh, SqnAct;
 {
   assume L[Net#a] == (1 * Base#L);
@@ -195,8 +207,11 @@ procedure Net#anon$2#exit#4()
   assume 0 <= R[Net#c];
   assume 0 <= C[Net#c];
   assume R[Net#c] == 0;
-  assume (forall idx$: int :: 
-    (0 <= idx$) && (idx$ < L[Net#a]) ==> (0 <= M[Net#a][idx$]) && (0 <= M[Net#b][idx$])
+  assume (forall i: int :: 
+    (0 <= i) && (i < L[Net#a]) ==> (0 <= M[Net#a][i])
+  );
+  assume (forall i: int :: 
+    (0 <= i) && (i < L[Net#b]) ==> (0 <= M[Net#b][i])
   );
   assume R[Net#a] == (R[Net#c] + C[Net#c]);
   assume R[Net#b] == (R[Net#c] + C[Net#c]);
@@ -219,15 +234,15 @@ procedure Net#anon$2#exit#4()
   assume !((R[Net#a] + C[Net#a]) < L[Net#a]);
   assume !((R[Net#b] + C[Net#b]) < L[Net#b]);
   assume !((1 <= C[Net#a]) && (1 <= C[Net#b]));
-  assert {:msg "  12.13: Network action postcondition might not hold"} (forall idx$: int :: 
-    (0 <= idx$) && (idx$ < L[Net#a]) ==> (M[Net#c][0] == (M[Net#a][idx$] + M[Net#b][idx$]))
+  assert {:msg "  13.14: Network action postcondition might not hold"} (forall i: int :: 
+    (0 <= i) && (i < (R[Net#c] + C[Net#c])) ==> (0 <= M[Net#c][i])
   );
-  assert {:msg "  13.13: Network action postcondition might not hold"} (forall idx$: int :: 
-    (0 <= idx$) && (idx$ < L[Net#a]) ==> (SqnCh[Net#c][0] == 0)
+  assert {:msg "  14.14: Network action postcondition might not hold"} (forall i: int :: 
+    (0 <= i) && (i < (R[Net#c] + C[Net#c])) ==> (SqnCh[Net#c][i] == i)
   );
   R[Net#c] := R[Net#c] + C[Net#c];
   C[Net#c] := C[Net#c] - (1 * Base#L);
-  assert {:msg "  The network might leave unread tokens on channel a"} C[Net#a] == 0;
-  assert {:msg "  The network might leave unread tokens on channel b"} C[Net#b] == 0;
-  assert {:msg "  The network might not produce the specified number of tokens on output out"} C[Net#c] == 0;
+  assert {:msg "  10.3: The network might leave unread tokens on channel a"} C[Net#a] == 0;
+  assert {:msg "  10.3: The network might leave unread tokens on channel b"} C[Net#b] == 0;
+  assert {:msg "  10.3: The network might not produce the specified number of tokens on output out"} C[Net#c] == 0;
 }
