ft_tests/Timeout.bpl
@@ -56,7 +56,7 @@ procedure Adjudicator#normal#2()
   var y: Chan (int);
   var c_out: Chan (int);
   assume true;
-  assume (M[x1][0] == M[x2][0]) && (M[x1][0] == M[c_in][0]);
+  assume (SqnCh[x1][0] == SqnCh[x2][0]) && (SqnCh[x1][0] == M[c_in][0]);
   assume true;
 }
 procedure Adjudicator#timeout#3()
@@ -79,10 +79,21 @@ procedure Adjudicator#readoff#4()
   var y: Chan (int);
   var c_out: Chan (int);
   assume true;
-  assume M[x1][0] < M[c_in][0];
+  assume SqnCh[x1][0] < M[c_in][0];
   assume true;
 }
-procedure Net#init#5()
+procedure Adjudicator#anon$2#5()
+  modifies C, R, M, St, SqnCh, SqnAct;
+{
+  var x1: Chan (int);
+  var x2: Chan (int);
+  var c_in: Chan (int);
+  var y: Chan (int);
+  var c_out: Chan (int);
+  assume true;
+  assume true;
+}
+procedure Net#init#6()
   modifies C, R, M, St, SqnCh, SqnAct;
 {
   assume C[Net#a] == 0;
@@ -99,8 +110,10 @@ procedure Net#init#5()
   assume R[Net#f] == 0;
   assume C[Net#g] == 0;
   assume R[Net#g] == 0;
+  M[Net#f][R[Net#f] + C[Net#f]] := 0;
+  C[Net#f] := C[Net#f] + 1;
   C[Net#f] := C[Net#f] - 1;
-  assume M[Net#f][R[Net#f]] == 0;
+  assert {:msg "  38.13: Network initialization might not establish the network invariant"} R[Net#e] == M[Net#f][R[Net#f]];
 }
 const unique Net#spl: Actor;
 const unique Net#pri: Actor;
@@ -113,17 +126,14 @@ const unique Net#d: Chan (int);
 const unique Net#e: Chan (int);
 const unique Net#f: Chan (int);
 const unique Net#g: Chan (int);
-procedure Net#anon$2#entry#6()
+procedure Net#anon$3#entry#7()
   modifies C, R, M, St, SqnCh, SqnAct;
 {
-  var ActionPH#y1: int;
-  var ActionPH#y2: int;
-  var ActionPH#y3: int;
   assume SqnAct[Net#spl] == 0;
   assume SqnAct[Net#pri] == 0;
   assume SqnAct[Net#sec] == 0;
   assume SqnAct[Net#adj] == 0;
-  assume L[Net#a] == (3 * Base#L);
+  assume L[Net#a] == (1 * Base#L);
   assume R[Net#a] == 0;
   assume C[Net#a] == 0;
   assume R[Net#b] == 0;
@@ -139,8 +149,8 @@ procedure Net#anon$2#entry#6()
   assume R[Net#g] == 0;
   assume C[Net#g] == 0;
   C[Net#f] := C[Net#f] + 1;
-  assume M[Net#f][R[Net#f]] == 0;
-  assume (M[Net#a][0] == 0) && (M[Net#a][1] == 1) && (M[Net#a][2] == 2);
+  assume R[Net#e] == M[Net#f][R[Net#f]];
+  assert {:msg "  38.13: Invariant might not hold"} R[Net#e] == M[Net#f][R[Net#f]];
   assume 0 <= R[Net#a];
   assume 0 <= C[Net#a];
   assume (R[Net#a] + C[Net#a]) <= L[Net#a];
@@ -157,45 +167,64 @@ procedure Net#anon$2#entry#6()
   assume 0 <= R[Net#g];
   assume 0 <= C[Net#g];
   assume R[Net#g] == 0;
-  assert {:msg "  Channel invariant might not hold on action entry (#16)"} (M[Net#a][0] == 0) && (M[Net#a][1] == 1) && (M[Net#a][2] == 2);
-  assert {:msg "  Channel invariant might not hold on action entry (#17)"} R[Net#a] == (R[Net#b] + C[Net#b]);
-  assert {:msg "  Channel invariant might not hold on action entry (#18)"} R[Net#a] == (R[Net#c] + C[Net#c]);
-  assert {:msg "  Channel invariant might not hold on action entry (#19)"} R[Net#b] == (R[Net#d] + C[Net#d]);
-  assert {:msg "  Channel invariant might not hold on action entry (#20)"} R[Net#c] == (R[Net#e] + C[Net#e]);
-  assert {:msg "  Channel invariant might not hold on action entry (#21)"} (forall idx$: int :: 
+  assert {:msg "  Channel invariant might not hold on action entry (#16)"} R[Net#a] == (R[Net#b] + C[Net#b]);
+  assert {:msg "  Channel invariant might not hold on action entry (#17)"} R[Net#a] == (R[Net#c] + C[Net#c]);
+  assert {:msg "  Channel invariant might not hold on action entry (#18)"} R[Net#b] == (R[Net#d] + C[Net#d]);
+  assert {:msg "  Channel invariant might not hold on action entry (#19)"} R[Net#c] == (R[Net#e] + C[Net#e]);
+  assert {:msg "  Channel invariant might not hold on action entry (#20)"} (forall idx$: int :: 
     (0 <= idx$) && (idx$ < (R[Net#b] + C[Net#b])) ==> (M[Net#b][idx$] == M[Net#a][idx$])
   );
-  assert {:msg "  Channel invariant might not hold on action entry (#22)"} (forall idx$: int :: 
+  assert {:msg "  Channel invariant might not hold on action entry (#21)"} (forall idx$: int :: 
     (0 <= idx$) && (idx$ < (R[Net#c] + C[Net#c])) ==> (M[Net#c][idx$] == M[Net#a][idx$])
   );
-  assert {:msg "  Channel invariant might not hold on action entry (#23)"} (forall idx$: int :: 
+  assert {:msg "  Channel invariant might not hold on action entry (#22)"} (forall idx$: int :: 
     (0 <= idx$) && (idx$ < (R[Net#d] + C[Net#d])) ==> (M[Net#d][idx$] == M[Net#b][idx$])
   );
-  assert {:msg "  Channel invariant might not hold on action entry (#24)"} (forall idx$: int :: 
+  assert {:msg "  Channel invariant might not hold on action entry (#23)"} (forall idx$: int :: 
     (0 <= idx$) && (idx$ < (R[Net#e] + C[Net#e])) ==> (M[Net#e][idx$] == M[Net#c][idx$])
   );
-  assert {:msg "  Channel invariant might not hold on action entry (#25)"} (forall idx$: int :: 
+  assert {:msg "  Channel invariant might not hold on action entry (#24)"} (forall idx$: int :: 
     (0 <= idx$) && (idx$ < (R[Net#a] + C[Net#a])) ==> (SqnCh[Net#a][idx$] == idx$)
   );
-  assert {:msg "  40.3: Channel invariant might not hold on action entry (#26)"} (R[Net#a] + C[Net#a]) <= 3;
-  assert {:msg "  47.3: Channel invariant might not hold on action entry (#27)"} C[Net#f] == 1;
-  assert {:msg "  48.3: Channel invariant might not hold on action entry (#28)"} C[Net#g] == R[Net#e];
-  assert {:msg "  49.3: Channel invariant might not hold on action entry (#29)"} R[Net#e] == M[Net#f][R[Net#f]];
-  assert {:msg "  50.3: Channel invariant might not hold on action entry (#30)"} R[Net#d] <= R[Net#e];
-  assert {:msg "  51.3: Channel invariant might not hold on action entry (#31)"} (0 < R[Net#d]) && (0 < R[Net#e]) ==> (M[Net#d][R[Net#d] - 1] <= M[Net#e][R[Net#e] - 1]);
-  assert {:msg "  52.3: Channel invariant might not hold on action entry (#32)"} (forall i: int :: 
+  assert {:msg "  40.3: Channel invariant might not hold on action entry (#25)"} SqnAct[Net#spl] == R[Net#a];
+  assert {:msg "  41.3: Channel invariant might not hold on action entry (#26)"} SqnAct[Net#pri] == R[Net#b];
+  assert {:msg "  42.3: Channel invariant might not hold on action entry (#27)"} SqnAct[Net#sec] == R[Net#c];
+  assert {:msg "  43.3: Channel invariant might not hold on action entry (#28)"} SqnAct[Net#adj] == R[Net#e];
+  assert {:msg "  45.3: Channel invariant might not hold on action entry (#29)"} (forall i: int :: 
+    (0 <= i) && (i < (R[Net#a] + C[Net#a])) ==> (SqnCh[Net#a][i] == i)
+  );
+  assert {:msg "  46.3: Channel invariant might not hold on action entry (#30)"} (forall i: int :: 
+    (0 <= i) && (i < (R[Net#b] + C[Net#b])) ==> (SqnCh[Net#b][i] == i)
+  );
+  assert {:msg "  47.3: Channel invariant might not hold on action entry (#31)"} (forall i: int :: 
+    (0 <= i) && (i < (R[Net#c] + C[Net#c])) ==> (SqnCh[Net#c][i] == i)
+  );
+  assert {:msg "  48.3: Channel invariant might not hold on action entry (#32)"} (forall i: int :: 
+    (0 <= i) && (i < (R[Net#d] + C[Net#d])) ==> (SqnCh[Net#d][i] == i)
+  );
+  assert {:msg "  49.3: Channel invariant might not hold on action entry (#33)"} (forall i: int :: 
+    (0 <= i) && (i < (R[Net#e] + C[Net#e])) ==> (SqnCh[Net#e][i] == i)
+  );
+  assert {:msg "  50.3: Channel invariant might not hold on action entry (#34)"} (forall i: int :: 
+    (0 <= i) && (i < (R[Net#g] + C[Net#g])) ==> (SqnCh[Net#g][i] == i)
+  );
+  assert {:msg "  52.3: Channel invariant might not hold on action entry (#35)"} C[Net#f] == 1;
+  assert {:msg "  53.3: Channel invariant might not hold on action entry (#36)"} C[Net#g] == R[Net#e];
+  assert {:msg "  54.3: Channel invariant might not hold on action entry (#37)"} R[Net#e] == M[Net#f][R[Net#f]];
+  assert {:msg "  55.3: Channel invariant might not hold on action entry (#38)"} (forall i: int :: 
+    (0 <= i) && (i < (R[Net#g] + C[Net#g])) ==> (SqnCh[Net#g][i] == i)
+  );
+  assert {:msg "  59.3: Channel invariant might not hold on action entry (#39)"} (0 < R[Net#d]) && (0 < R[Net#e]) ==> (M[Net#d][R[Net#d] - 1] <= M[Net#e][R[Net#e] - 1]);
+  assert {:msg "  60.3: Channel invariant might not hold on action entry (#40)"} (forall i: int :: 
     (0 <= i) && (i < R[Net#e]) ==> (M[Net#g][i] == M[Net#e][i])
   );
 }
-procedure Net#anon$2#Split#anon$1#7()
+procedure Net#anon$3#Split#anon$1#8()
   modifies C, R, M, St, SqnCh, SqnAct;
 {
-  var ActionPH#y1: int;
-  var ActionPH#y2: int;
-  var ActionPH#y3: int;
   var St#next: State;
   var in#i: int;
-  assume L[Net#a] == (3 * Base#L);
+  assume L[Net#a] == (1 * Base#L);
   assume 0 <= R[Net#a];
   assume 0 <= C[Net#a];
   assume (R[Net#a] + C[Net#a]) <= L[Net#a];
@@ -212,7 +241,6 @@ procedure Net#anon$2#Split#anon$1#7()
   assume 0 <= R[Net#g];
   assume 0 <= C[Net#g];
   assume R[Net#g] == 0;
-  assume (M[Net#a][0] == 0) && (M[Net#a][1] == 1) && (M[Net#a][2] == 2);
   assume R[Net#a] == (R[Net#b] + C[Net#b]);
   assume R[Net#a] == (R[Net#c] + C[Net#c]);
   assume R[Net#b] == (R[Net#d] + C[Net#d]);
@@ -232,11 +260,34 @@ procedure Net#anon$2#Split#anon$1#7()
   assume (forall idx$: int :: 
     (0 <= idx$) && (idx$ < (R[Net#a] + C[Net#a])) ==> (SqnCh[Net#a][idx$] == idx$)
   );
-  assume (R[Net#a] + C[Net#a]) <= 3;
+  assume SqnAct[Net#spl] == R[Net#a];
+  assume SqnAct[Net#pri] == R[Net#b];
+  assume SqnAct[Net#sec] == R[Net#c];
+  assume SqnAct[Net#adj] == R[Net#e];
+  assume (forall i: int :: 
+    (0 <= i) && (i < (R[Net#a] + C[Net#a])) ==> (SqnCh[Net#a][i] == i)
+  );
+  assume (forall i: int :: 
+    (0 <= i) && (i < (R[Net#b] + C[Net#b])) ==> (SqnCh[Net#b][i] == i)
+  );
+  assume (forall i: int :: 
+    (0 <= i) && (i < (R[Net#c] + C[Net#c])) ==> (SqnCh[Net#c][i] == i)
+  );
+  assume (forall i: int :: 
+    (0 <= i) && (i < (R[Net#d] + C[Net#d])) ==> (SqnCh[Net#d][i] == i)
+  );
+  assume (forall i: int :: 
+    (0 <= i) && (i < (R[Net#e] + C[Net#e])) ==> (SqnCh[Net#e][i] == i)
+  );
+  assume (forall i: int :: 
+    (0 <= i) && (i < (R[Net#g] + C[Net#g])) ==> (SqnCh[Net#g][i] == i)
+  );
   assume C[Net#f] == 1;
   assume C[Net#g] == R[Net#e];
   assume R[Net#e] == M[Net#f][R[Net#f]];
-  assume R[Net#d] <= R[Net#e];
+  assume (forall i: int :: 
+    (0 <= i) && (i < (R[Net#g] + C[Net#g])) ==> (SqnCh[Net#g][i] == i)
+  );
   assume (0 < R[Net#d]) && (0 < R[Net#e]) ==> (M[Net#d][R[Net#d] - 1] <= M[Net#e][R[Net#e] - 1]);
   assume (forall i: int :: 
     (0 <= i) && (i < R[Net#e]) ==> (M[Net#g][i] == M[Net#e][i])
@@ -269,45 +320,64 @@ procedure Net#anon$2#Split#anon$1#7()
   assume 0 <= R[Net#g];
   assume 0 <= C[Net#g];
   assume R[Net#g] == 0;
-  assert {:msg "  Action at 8.3 ('anon$1') for actor instance 'spl' might not preserve the channel invariant (#49)"} (M[Net#a][0] == 0) && (M[Net#a][1] == 1) && (M[Net#a][2] == 2);
-  assert {:msg "  Action at 8.3 ('anon$1') for actor instance 'spl' might not preserve the channel invariant (#50)"} R[Net#a] == (R[Net#b] + C[Net#b]);
-  assert {:msg "  Action at 8.3 ('anon$1') for actor instance 'spl' might not preserve the channel invariant (#51)"} R[Net#a] == (R[Net#c] + C[Net#c]);
-  assert {:msg "  Action at 8.3 ('anon$1') for actor instance 'spl' might not preserve the channel invariant (#52)"} R[Net#b] == (R[Net#d] + C[Net#d]);
-  assert {:msg "  Action at 8.3 ('anon$1') for actor instance 'spl' might not preserve the channel invariant (#53)"} R[Net#c] == (R[Net#e] + C[Net#e]);
-  assert {:msg "  Action at 8.3 ('anon$1') for actor instance 'spl' might not preserve the channel invariant (#54)"} (forall idx$: int :: 
+  assert {:msg "  Action at 8.3 ('anon$1') for actor instance 'spl' might not preserve the channel invariant (#57)"} R[Net#a] == (R[Net#b] + C[Net#b]);
+  assert {:msg "  Action at 8.3 ('anon$1') for actor instance 'spl' might not preserve the channel invariant (#58)"} R[Net#a] == (R[Net#c] + C[Net#c]);
+  assert {:msg "  Action at 8.3 ('anon$1') for actor instance 'spl' might not preserve the channel invariant (#59)"} R[Net#b] == (R[Net#d] + C[Net#d]);
+  assert {:msg "  Action at 8.3 ('anon$1') for actor instance 'spl' might not preserve the channel invariant (#60)"} R[Net#c] == (R[Net#e] + C[Net#e]);
+  assert {:msg "  Action at 8.3 ('anon$1') for actor instance 'spl' might not preserve the channel invariant (#61)"} (forall idx$: int :: 
     (0 <= idx$) && (idx$ < (R[Net#b] + C[Net#b])) ==> (M[Net#b][idx$] == M[Net#a][idx$])
   );
-  assert {:msg "  Action at 8.3 ('anon$1') for actor instance 'spl' might not preserve the channel invariant (#55)"} (forall idx$: int :: 
+  assert {:msg "  Action at 8.3 ('anon$1') for actor instance 'spl' might not preserve the channel invariant (#62)"} (forall idx$: int :: 
     (0 <= idx$) && (idx$ < (R[Net#c] + C[Net#c])) ==> (M[Net#c][idx$] == M[Net#a][idx$])
   );
-  assert {:msg "  Action at 8.3 ('anon$1') for actor instance 'spl' might not preserve the channel invariant (#56)"} (forall idx$: int :: 
+  assert {:msg "  Action at 8.3 ('anon$1') for actor instance 'spl' might not preserve the channel invariant (#63)"} (forall idx$: int :: 
     (0 <= idx$) && (idx$ < (R[Net#d] + C[Net#d])) ==> (M[Net#d][idx$] == M[Net#b][idx$])
   );
-  assert {:msg "  Action at 8.3 ('anon$1') for actor instance 'spl' might not preserve the channel invariant (#57)"} (forall idx$: int :: 
+  assert {:msg "  Action at 8.3 ('anon$1') for actor instance 'spl' might not preserve the channel invariant (#64)"} (forall idx$: int :: 
     (0 <= idx$) && (idx$ < (R[Net#e] + C[Net#e])) ==> (M[Net#e][idx$] == M[Net#c][idx$])
   );
-  assert {:msg "  Action at 8.3 ('anon$1') for actor instance 'spl' might not preserve the channel invariant (#58)"} (forall idx$: int :: 
+  assert {:msg "  Action at 8.3 ('anon$1') for actor instance 'spl' might not preserve the channel invariant (#65)"} (forall idx$: int :: 
     (0 <= idx$) && (idx$ < (R[Net#a] + C[Net#a])) ==> (SqnCh[Net#a][idx$] == idx$)
   );
-  assert {:msg "  40.3: Action at 8.3 ('anon$1') for actor instance 'spl' might not preserve the channel invariant (#59)"} (R[Net#a] + C[Net#a]) <= 3;
-  assert {:msg "  47.3: Action at 8.3 ('anon$1') for actor instance 'spl' might not preserve the channel invariant (#60)"} C[Net#f] == 1;
-  assert {:msg "  48.3: Action at 8.3 ('anon$1') for actor instance 'spl' might not preserve the channel invariant (#61)"} C[Net#g] == R[Net#e];
-  assert {:msg "  49.3: Action at 8.3 ('anon$1') for actor instance 'spl' might not preserve the channel invariant (#62)"} R[Net#e] == M[Net#f][R[Net#f]];
-  assert {:msg "  50.3: Action at 8.3 ('anon$1') for actor instance 'spl' might not preserve the channel invariant (#63)"} R[Net#d] <= R[Net#e];
-  assert {:msg "  51.3: Action at 8.3 ('anon$1') for actor instance 'spl' might not preserve the channel invariant (#64)"} (0 < R[Net#d]) && (0 < R[Net#e]) ==> (M[Net#d][R[Net#d] - 1] <= M[Net#e][R[Net#e] - 1]);
-  assert {:msg "  52.3: Action at 8.3 ('anon$1') for actor instance 'spl' might not preserve the channel invariant (#65)"} (forall i: int :: 
+  assert {:msg "  40.3: Action at 8.3 ('anon$1') for actor instance 'spl' might not preserve the channel invariant (#66)"} SqnAct[Net#spl] == R[Net#a];
+  assert {:msg "  41.3: Action at 8.3 ('anon$1') for actor instance 'spl' might not preserve the channel invariant (#67)"} SqnAct[Net#pri] == R[Net#b];
+  assert {:msg "  42.3: Action at 8.3 ('anon$1') for actor instance 'spl' might not preserve the channel invariant (#68)"} SqnAct[Net#sec] == R[Net#c];
+  assert {:msg "  43.3: Action at 8.3 ('anon$1') for actor instance 'spl' might not preserve the channel invariant (#69)"} SqnAct[Net#adj] == R[Net#e];
+  assert {:msg "  45.3: Action at 8.3 ('anon$1') for actor instance 'spl' might not preserve the channel invariant (#70)"} (forall i: int :: 
+    (0 <= i) && (i < (R[Net#a] + C[Net#a])) ==> (SqnCh[Net#a][i] == i)
+  );
+  assert {:msg "  46.3: Action at 8.3 ('anon$1') for actor instance 'spl' might not preserve the channel invariant (#71)"} (forall i: int :: 
+    (0 <= i) && (i < (R[Net#b] + C[Net#b])) ==> (SqnCh[Net#b][i] == i)
+  );
+  assert {:msg "  47.3: Action at 8.3 ('anon$1') for actor instance 'spl' might not preserve the channel invariant (#72)"} (forall i: int :: 
+    (0 <= i) && (i < (R[Net#c] + C[Net#c])) ==> (SqnCh[Net#c][i] == i)
+  );
+  assert {:msg "  48.3: Action at 8.3 ('anon$1') for actor instance 'spl' might not preserve the channel invariant (#73)"} (forall i: int :: 
+    (0 <= i) && (i < (R[Net#d] + C[Net#d])) ==> (SqnCh[Net#d][i] == i)
+  );
+  assert {:msg "  49.3: Action at 8.3 ('anon$1') for actor instance 'spl' might not preserve the channel invariant (#74)"} (forall i: int :: 
+    (0 <= i) && (i < (R[Net#e] + C[Net#e])) ==> (SqnCh[Net#e][i] == i)
+  );
+  assert {:msg "  50.3: Action at 8.3 ('anon$1') for actor instance 'spl' might not preserve the channel invariant (#75)"} (forall i: int :: 
+    (0 <= i) && (i < (R[Net#g] + C[Net#g])) ==> (SqnCh[Net#g][i] == i)
+  );
+  assert {:msg "  52.3: Action at 8.3 ('anon$1') for actor instance 'spl' might not preserve the channel invariant (#76)"} C[Net#f] == 1;
+  assert {:msg "  53.3: Action at 8.3 ('anon$1') for actor instance 'spl' might not preserve the channel invariant (#77)"} C[Net#g] == R[Net#e];
+  assert {:msg "  54.3: Action at 8.3 ('anon$1') for actor instance 'spl' might not preserve the channel invariant (#78)"} R[Net#e] == M[Net#f][R[Net#f]];
+  assert {:msg "  55.3: Action at 8.3 ('anon$1') for actor instance 'spl' might not preserve the channel invariant (#79)"} (forall i: int :: 
+    (0 <= i) && (i < (R[Net#g] + C[Net#g])) ==> (SqnCh[Net#g][i] == i)
+  );
+  assert {:msg "  59.3: Action at 8.3 ('anon$1') for actor instance 'spl' might not preserve the channel invariant (#80)"} (0 < R[Net#d]) && (0 < R[Net#e]) ==> (M[Net#d][R[Net#d] - 1] <= M[Net#e][R[Net#e] - 1]);
+  assert {:msg "  60.3: Action at 8.3 ('anon$1') for actor instance 'spl' might not preserve the channel invariant (#81)"} (forall i: int :: 
     (0 <= i) && (i < R[Net#e]) ==> (M[Net#g][i] == M[Net#e][i])
   );
 }
-procedure Net#anon$2#Rep#anon$0#8()
+procedure Net#anon$3#Rep#anon$0#9()
   modifies C, R, M, St, SqnCh, SqnAct;
 {
-  var ActionPH#y1: int;
-  var ActionPH#y2: int;
-  var ActionPH#y3: int;
   var St#next: State;
   var in#i: int;
-  assume L[Net#a] == (3 * Base#L);
+  assume L[Net#a] == (1 * Base#L);
   assume 0 <= R[Net#a];
   assume 0 <= C[Net#a];
   assume (R[Net#a] + C[Net#a]) <= L[Net#a];
@@ -324,7 +394,6 @@ procedure Net#anon$2#Rep#anon$0#8()
   assume 0 <= R[Net#g];
   assume 0 <= C[Net#g];
   assume R[Net#g] == 0;
-  assume (M[Net#a][0] == 0) && (M[Net#a][1] == 1) && (M[Net#a][2] == 2);
   assume R[Net#a] == (R[Net#b] + C[Net#b]);
   assume R[Net#a] == (R[Net#c] + C[Net#c]);
   assume R[Net#b] == (R[Net#d] + C[Net#d]);
@@ -344,11 +413,34 @@ procedure Net#anon$2#Rep#anon$0#8()
   assume (forall idx$: int :: 
     (0 <= idx$) && (idx$ < (R[Net#a] + C[Net#a])) ==> (SqnCh[Net#a][idx$] == idx$)
   );
-  assume (R[Net#a] + C[Net#a]) <= 3;
+  assume SqnAct[Net#spl] == R[Net#a];
+  assume SqnAct[Net#pri] == R[Net#b];
+  assume SqnAct[Net#sec] == R[Net#c];
+  assume SqnAct[Net#adj] == R[Net#e];
+  assume (forall i: int :: 
+    (0 <= i) && (i < (R[Net#a] + C[Net#a])) ==> (SqnCh[Net#a][i] == i)
+  );
+  assume (forall i: int :: 
+    (0 <= i) && (i < (R[Net#b] + C[Net#b])) ==> (SqnCh[Net#b][i] == i)
+  );
+  assume (forall i: int :: 
+    (0 <= i) && (i < (R[Net#c] + C[Net#c])) ==> (SqnCh[Net#c][i] == i)
+  );
+  assume (forall i: int :: 
+    (0 <= i) && (i < (R[Net#d] + C[Net#d])) ==> (SqnCh[Net#d][i] == i)
+  );
+  assume (forall i: int :: 
+    (0 <= i) && (i < (R[Net#e] + C[Net#e])) ==> (SqnCh[Net#e][i] == i)
+  );
+  assume (forall i: int :: 
+    (0 <= i) && (i < (R[Net#g] + C[Net#g])) ==> (SqnCh[Net#g][i] == i)
+  );
   assume C[Net#f] == 1;
   assume C[Net#g] == R[Net#e];
   assume R[Net#e] == M[Net#f][R[Net#f]];
-  assume R[Net#d] <= R[Net#e];
+  assume (forall i: int :: 
+    (0 <= i) && (i < (R[Net#g] + C[Net#g])) ==> (SqnCh[Net#g][i] == i)
+  );
   assume (0 < R[Net#d]) && (0 < R[Net#e]) ==> (M[Net#d][R[Net#d] - 1] <= M[Net#e][R[Net#e] - 1]);
   assume (forall i: int :: 
     (0 <= i) && (i < R[Net#e]) ==> (M[Net#g][i] == M[Net#e][i])
@@ -378,45 +470,64 @@ procedure Net#anon$2#Rep#anon$0#8()
   assume 0 <= R[Net#g];
   assume 0 <= C[Net#g];
   assume R[Net#g] == 0;
-  assert {:msg "  Action at 3.3 ('anon$0') for actor instance 'pri' might not preserve the channel invariant (#82)"} (M[Net#a][0] == 0) && (M[Net#a][1] == 1) && (M[Net#a][2] == 2);
-  assert {:msg "  Action at 3.3 ('anon$0') for actor instance 'pri' might not preserve the channel invariant (#83)"} R[Net#a] == (R[Net#b] + C[Net#b]);
-  assert {:msg "  Action at 3.3 ('anon$0') for actor instance 'pri' might not preserve the channel invariant (#84)"} R[Net#a] == (R[Net#c] + C[Net#c]);
-  assert {:msg "  Action at 3.3 ('anon$0') for actor instance 'pri' might not preserve the channel invariant (#85)"} R[Net#b] == (R[Net#d] + C[Net#d]);
-  assert {:msg "  Action at 3.3 ('anon$0') for actor instance 'pri' might not preserve the channel invariant (#86)"} R[Net#c] == (R[Net#e] + C[Net#e]);
-  assert {:msg "  Action at 3.3 ('anon$0') for actor instance 'pri' might not preserve the channel invariant (#87)"} (forall idx$: int :: 
+  assert {:msg "  Action at 3.3 ('anon$0') for actor instance 'pri' might not preserve the channel invariant (#98)"} R[Net#a] == (R[Net#b] + C[Net#b]);
+  assert {:msg "  Action at 3.3 ('anon$0') for actor instance 'pri' might not preserve the channel invariant (#99)"} R[Net#a] == (R[Net#c] + C[Net#c]);
+  assert {:msg "  Action at 3.3 ('anon$0') for actor instance 'pri' might not preserve the channel invariant (#100)"} R[Net#b] == (R[Net#d] + C[Net#d]);
+  assert {:msg "  Action at 3.3 ('anon$0') for actor instance 'pri' might not preserve the channel invariant (#101)"} R[Net#c] == (R[Net#e] + C[Net#e]);
+  assert {:msg "  Action at 3.3 ('anon$0') for actor instance 'pri' might not preserve the channel invariant (#102)"} (forall idx$: int :: 
     (0 <= idx$) && (idx$ < (R[Net#b] + C[Net#b])) ==> (M[Net#b][idx$] == M[Net#a][idx$])
   );
-  assert {:msg "  Action at 3.3 ('anon$0') for actor instance 'pri' might not preserve the channel invariant (#88)"} (forall idx$: int :: 
+  assert {:msg "  Action at 3.3 ('anon$0') for actor instance 'pri' might not preserve the channel invariant (#103)"} (forall idx$: int :: 
     (0 <= idx$) && (idx$ < (R[Net#c] + C[Net#c])) ==> (M[Net#c][idx$] == M[Net#a][idx$])
   );
-  assert {:msg "  Action at 3.3 ('anon$0') for actor instance 'pri' might not preserve the channel invariant (#89)"} (forall idx$: int :: 
+  assert {:msg "  Action at 3.3 ('anon$0') for actor instance 'pri' might not preserve the channel invariant (#104)"} (forall idx$: int :: 
     (0 <= idx$) && (idx$ < (R[Net#d] + C[Net#d])) ==> (M[Net#d][idx$] == M[Net#b][idx$])
   );
-  assert {:msg "  Action at 3.3 ('anon$0') for actor instance 'pri' might not preserve the channel invariant (#90)"} (forall idx$: int :: 
+  assert {:msg "  Action at 3.3 ('anon$0') for actor instance 'pri' might not preserve the channel invariant (#105)"} (forall idx$: int :: 
     (0 <= idx$) && (idx$ < (R[Net#e] + C[Net#e])) ==> (M[Net#e][idx$] == M[Net#c][idx$])
   );
-  assert {:msg "  Action at 3.3 ('anon$0') for actor instance 'pri' might not preserve the channel invariant (#91)"} (forall idx$: int :: 
+  assert {:msg "  Action at 3.3 ('anon$0') for actor instance 'pri' might not preserve the channel invariant (#106)"} (forall idx$: int :: 
     (0 <= idx$) && (idx$ < (R[Net#a] + C[Net#a])) ==> (SqnCh[Net#a][idx$] == idx$)
   );
-  assert {:msg "  40.3: Action at 3.3 ('anon$0') for actor instance 'pri' might not preserve the channel invariant (#92)"} (R[Net#a] + C[Net#a]) <= 3;
-  assert {:msg "  47.3: Action at 3.3 ('anon$0') for actor instance 'pri' might not preserve the channel invariant (#93)"} C[Net#f] == 1;
-  assert {:msg "  48.3: Action at 3.3 ('anon$0') for actor instance 'pri' might not preserve the channel invariant (#94)"} C[Net#g] == R[Net#e];
-  assert {:msg "  49.3: Action at 3.3 ('anon$0') for actor instance 'pri' might not preserve the channel invariant (#95)"} R[Net#e] == M[Net#f][R[Net#f]];
-  assert {:msg "  50.3: Action at 3.3 ('anon$0') for actor instance 'pri' might not preserve the channel invariant (#96)"} R[Net#d] <= R[Net#e];
-  assert {:msg "  51.3: Action at 3.3 ('anon$0') for actor instance 'pri' might not preserve the channel invariant (#97)"} (0 < R[Net#d]) && (0 < R[Net#e]) ==> (M[Net#d][R[Net#d] - 1] <= M[Net#e][R[Net#e] - 1]);
-  assert {:msg "  52.3: Action at 3.3 ('anon$0') for actor instance 'pri' might not preserve the channel invariant (#98)"} (forall i: int :: 
+  assert {:msg "  40.3: Action at 3.3 ('anon$0') for actor instance 'pri' might not preserve the channel invariant (#107)"} SqnAct[Net#spl] == R[Net#a];
+  assert {:msg "  41.3: Action at 3.3 ('anon$0') for actor instance 'pri' might not preserve the channel invariant (#108)"} SqnAct[Net#pri] == R[Net#b];
+  assert {:msg "  42.3: Action at 3.3 ('anon$0') for actor instance 'pri' might not preserve the channel invariant (#109)"} SqnAct[Net#sec] == R[Net#c];
+  assert {:msg "  43.3: Action at 3.3 ('anon$0') for actor instance 'pri' might not preserve the channel invariant (#110)"} SqnAct[Net#adj] == R[Net#e];
+  assert {:msg "  45.3: Action at 3.3 ('anon$0') for actor instance 'pri' might not preserve the channel invariant (#111)"} (forall i: int :: 
+    (0 <= i) && (i < (R[Net#a] + C[Net#a])) ==> (SqnCh[Net#a][i] == i)
+  );
+  assert {:msg "  46.3: Action at 3.3 ('anon$0') for actor instance 'pri' might not preserve the channel invariant (#112)"} (forall i: int :: 
+    (0 <= i) && (i < (R[Net#b] + C[Net#b])) ==> (SqnCh[Net#b][i] == i)
+  );
+  assert {:msg "  47.3: Action at 3.3 ('anon$0') for actor instance 'pri' might not preserve the channel invariant (#113)"} (forall i: int :: 
+    (0 <= i) && (i < (R[Net#c] + C[Net#c])) ==> (SqnCh[Net#c][i] == i)
+  );
+  assert {:msg "  48.3: Action at 3.3 ('anon$0') for actor instance 'pri' might not preserve the channel invariant (#114)"} (forall i: int :: 
+    (0 <= i) && (i < (R[Net#d] + C[Net#d])) ==> (SqnCh[Net#d][i] == i)
+  );
+  assert {:msg "  49.3: Action at 3.3 ('anon$0') for actor instance 'pri' might not preserve the channel invariant (#115)"} (forall i: int :: 
+    (0 <= i) && (i < (R[Net#e] + C[Net#e])) ==> (SqnCh[Net#e][i] == i)
+  );
+  assert {:msg "  50.3: Action at 3.3 ('anon$0') for actor instance 'pri' might not preserve the channel invariant (#116)"} (forall i: int :: 
+    (0 <= i) && (i < (R[Net#g] + C[Net#g])) ==> (SqnCh[Net#g][i] == i)
+  );
+  assert {:msg "  52.3: Action at 3.3 ('anon$0') for actor instance 'pri' might not preserve the channel invariant (#117)"} C[Net#f] == 1;
+  assert {:msg "  53.3: Action at 3.3 ('anon$0') for actor instance 'pri' might not preserve the channel invariant (#118)"} C[Net#g] == R[Net#e];
+  assert {:msg "  54.3: Action at 3.3 ('anon$0') for actor instance 'pri' might not preserve the channel invariant (#119)"} R[Net#e] == M[Net#f][R[Net#f]];
+  assert {:msg "  55.3: Action at 3.3 ('anon$0') for actor instance 'pri' might not preserve the channel invariant (#120)"} (forall i: int :: 
+    (0 <= i) && (i < (R[Net#g] + C[Net#g])) ==> (SqnCh[Net#g][i] == i)
+  );
+  assert {:msg "  59.3: Action at 3.3 ('anon$0') for actor instance 'pri' might not preserve the channel invariant (#121)"} (0 < R[Net#d]) && (0 < R[Net#e]) ==> (M[Net#d][R[Net#d] - 1] <= M[Net#e][R[Net#e] - 1]);
+  assert {:msg "  60.3: Action at 3.3 ('anon$0') for actor instance 'pri' might not preserve the channel invariant (#122)"} (forall i: int :: 
     (0 <= i) && (i < R[Net#e]) ==> (M[Net#g][i] == M[Net#e][i])
   );
 }
-procedure Net#anon$2#Rep#anon$0#9()
+procedure Net#anon$3#Rep#anon$0#10()
   modifies C, R, M, St, SqnCh, SqnAct;
 {
-  var ActionPH#y1: int;
-  var ActionPH#y2: int;
-  var ActionPH#y3: int;
   var St#next: State;
   var in#i: int;
-  assume L[Net#a] == (3 * Base#L);
+  assume L[Net#a] == (1 * Base#L);
   assume 0 <= R[Net#a];
   assume 0 <= C[Net#a];
   assume (R[Net#a] + C[Net#a]) <= L[Net#a];
@@ -433,7 +544,6 @@ procedure Net#anon$2#Rep#anon$0#9()
   assume 0 <= R[Net#g];
   assume 0 <= C[Net#g];
   assume R[Net#g] == 0;
-  assume (M[Net#a][0] == 0) && (M[Net#a][1] == 1) && (M[Net#a][2] == 2);
   assume R[Net#a] == (R[Net#b] + C[Net#b]);
   assume R[Net#a] == (R[Net#c] + C[Net#c]);
   assume R[Net#b] == (R[Net#d] + C[Net#d]);
@@ -453,11 +563,34 @@ procedure Net#anon$2#Rep#anon$0#9()
   assume (forall idx$: int :: 
     (0 <= idx$) && (idx$ < (R[Net#a] + C[Net#a])) ==> (SqnCh[Net#a][idx$] == idx$)
   );
-  assume (R[Net#a] + C[Net#a]) <= 3;
+  assume SqnAct[Net#spl] == R[Net#a];
+  assume SqnAct[Net#pri] == R[Net#b];
+  assume SqnAct[Net#sec] == R[Net#c];
+  assume SqnAct[Net#adj] == R[Net#e];
+  assume (forall i: int :: 
+    (0 <= i) && (i < (R[Net#a] + C[Net#a])) ==> (SqnCh[Net#a][i] == i)
+  );
+  assume (forall i: int :: 
+    (0 <= i) && (i < (R[Net#b] + C[Net#b])) ==> (SqnCh[Net#b][i] == i)
+  );
+  assume (forall i: int :: 
+    (0 <= i) && (i < (R[Net#c] + C[Net#c])) ==> (SqnCh[Net#c][i] == i)
+  );
+  assume (forall i: int :: 
+    (0 <= i) && (i < (R[Net#d] + C[Net#d])) ==> (SqnCh[Net#d][i] == i)
+  );
+  assume (forall i: int :: 
+    (0 <= i) && (i < (R[Net#e] + C[Net#e])) ==> (SqnCh[Net#e][i] == i)
+  );
+  assume (forall i: int :: 
+    (0 <= i) && (i < (R[Net#g] + C[Net#g])) ==> (SqnCh[Net#g][i] == i)
+  );
   assume C[Net#f] == 1;
   assume C[Net#g] == R[Net#e];
   assume R[Net#e] == M[Net#f][R[Net#f]];
-  assume R[Net#d] <= R[Net#e];
+  assume (forall i: int :: 
+    (0 <= i) && (i < (R[Net#g] + C[Net#g])) ==> (SqnCh[Net#g][i] == i)
+  );
   assume (0 < R[Net#d]) && (0 < R[Net#e]) ==> (M[Net#d][R[Net#d] - 1] <= M[Net#e][R[Net#e] - 1]);
   assume (forall i: int :: 
     (0 <= i) && (i < R[Net#e]) ==> (M[Net#g][i] == M[Net#e][i])
@@ -487,46 +620,65 @@ procedure Net#anon$2#Rep#anon$0#9()
   assume 0 <= R[Net#g];
   assume 0 <= C[Net#g];
   assume R[Net#g] == 0;
-  assert {:msg "  Action at 3.3 ('anon$0') for actor instance 'sec' might not preserve the channel invariant (#115)"} (M[Net#a][0] == 0) && (M[Net#a][1] == 1) && (M[Net#a][2] == 2);
-  assert {:msg "  Action at 3.3 ('anon$0') for actor instance 'sec' might not preserve the channel invariant (#116)"} R[Net#a] == (R[Net#b] + C[Net#b]);
-  assert {:msg "  Action at 3.3 ('anon$0') for actor instance 'sec' might not preserve the channel invariant (#117)"} R[Net#a] == (R[Net#c] + C[Net#c]);
-  assert {:msg "  Action at 3.3 ('anon$0') for actor instance 'sec' might not preserve the channel invariant (#118)"} R[Net#b] == (R[Net#d] + C[Net#d]);
-  assert {:msg "  Action at 3.3 ('anon$0') for actor instance 'sec' might not preserve the channel invariant (#119)"} R[Net#c] == (R[Net#e] + C[Net#e]);
-  assert {:msg "  Action at 3.3 ('anon$0') for actor instance 'sec' might not preserve the channel invariant (#120)"} (forall idx$: int :: 
+  assert {:msg "  Action at 3.3 ('anon$0') for actor instance 'sec' might not preserve the channel invariant (#139)"} R[Net#a] == (R[Net#b] + C[Net#b]);
+  assert {:msg "  Action at 3.3 ('anon$0') for actor instance 'sec' might not preserve the channel invariant (#140)"} R[Net#a] == (R[Net#c] + C[Net#c]);
+  assert {:msg "  Action at 3.3 ('anon$0') for actor instance 'sec' might not preserve the channel invariant (#141)"} R[Net#b] == (R[Net#d] + C[Net#d]);
+  assert {:msg "  Action at 3.3 ('anon$0') for actor instance 'sec' might not preserve the channel invariant (#142)"} R[Net#c] == (R[Net#e] + C[Net#e]);
+  assert {:msg "  Action at 3.3 ('anon$0') for actor instance 'sec' might not preserve the channel invariant (#143)"} (forall idx$: int :: 
     (0 <= idx$) && (idx$ < (R[Net#b] + C[Net#b])) ==> (M[Net#b][idx$] == M[Net#a][idx$])
   );
-  assert {:msg "  Action at 3.3 ('anon$0') for actor instance 'sec' might not preserve the channel invariant (#121)"} (forall idx$: int :: 
+  assert {:msg "  Action at 3.3 ('anon$0') for actor instance 'sec' might not preserve the channel invariant (#144)"} (forall idx$: int :: 
     (0 <= idx$) && (idx$ < (R[Net#c] + C[Net#c])) ==> (M[Net#c][idx$] == M[Net#a][idx$])
   );
-  assert {:msg "  Action at 3.3 ('anon$0') for actor instance 'sec' might not preserve the channel invariant (#122)"} (forall idx$: int :: 
+  assert {:msg "  Action at 3.3 ('anon$0') for actor instance 'sec' might not preserve the channel invariant (#145)"} (forall idx$: int :: 
     (0 <= idx$) && (idx$ < (R[Net#d] + C[Net#d])) ==> (M[Net#d][idx$] == M[Net#b][idx$])
   );
-  assert {:msg "  Action at 3.3 ('anon$0') for actor instance 'sec' might not preserve the channel invariant (#123)"} (forall idx$: int :: 
+  assert {:msg "  Action at 3.3 ('anon$0') for actor instance 'sec' might not preserve the channel invariant (#146)"} (forall idx$: int :: 
     (0 <= idx$) && (idx$ < (R[Net#e] + C[Net#e])) ==> (M[Net#e][idx$] == M[Net#c][idx$])
   );
-  assert {:msg "  Action at 3.3 ('anon$0') for actor instance 'sec' might not preserve the channel invariant (#124)"} (forall idx$: int :: 
+  assert {:msg "  Action at 3.3 ('anon$0') for actor instance 'sec' might not preserve the channel invariant (#147)"} (forall idx$: int :: 
     (0 <= idx$) && (idx$ < (R[Net#a] + C[Net#a])) ==> (SqnCh[Net#a][idx$] == idx$)
   );
-  assert {:msg "  40.3: Action at 3.3 ('anon$0') for actor instance 'sec' might not preserve the channel invariant (#125)"} (R[Net#a] + C[Net#a]) <= 3;
-  assert {:msg "  47.3: Action at 3.3 ('anon$0') for actor instance 'sec' might not preserve the channel invariant (#126)"} C[Net#f] == 1;
-  assert {:msg "  48.3: Action at 3.3 ('anon$0') for actor instance 'sec' might not preserve the channel invariant (#127)"} C[Net#g] == R[Net#e];
-  assert {:msg "  49.3: Action at 3.3 ('anon$0') for actor instance 'sec' might not preserve the channel invariant (#128)"} R[Net#e] == M[Net#f][R[Net#f]];
-  assert {:msg "  50.3: Action at 3.3 ('anon$0') for actor instance 'sec' might not preserve the channel invariant (#129)"} R[Net#d] <= R[Net#e];
-  assert {:msg "  51.3: Action at 3.3 ('anon$0') for actor instance 'sec' might not preserve the channel invariant (#130)"} (0 < R[Net#d]) && (0 < R[Net#e]) ==> (M[Net#d][R[Net#d] - 1] <= M[Net#e][R[Net#e] - 1]);
-  assert {:msg "  52.3: Action at 3.3 ('anon$0') for actor instance 'sec' might not preserve the channel invariant (#131)"} (forall i: int :: 
+  assert {:msg "  40.3: Action at 3.3 ('anon$0') for actor instance 'sec' might not preserve the channel invariant (#148)"} SqnAct[Net#spl] == R[Net#a];
+  assert {:msg "  41.3: Action at 3.3 ('anon$0') for actor instance 'sec' might not preserve the channel invariant (#149)"} SqnAct[Net#pri] == R[Net#b];
+  assert {:msg "  42.3: Action at 3.3 ('anon$0') for actor instance 'sec' might not preserve the channel invariant (#150)"} SqnAct[Net#sec] == R[Net#c];
+  assert {:msg "  43.3: Action at 3.3 ('anon$0') for actor instance 'sec' might not preserve the channel invariant (#151)"} SqnAct[Net#adj] == R[Net#e];
+  assert {:msg "  45.3: Action at 3.3 ('anon$0') for actor instance 'sec' might not preserve the channel invariant (#152)"} (forall i: int :: 
+    (0 <= i) && (i < (R[Net#a] + C[Net#a])) ==> (SqnCh[Net#a][i] == i)
+  );
+  assert {:msg "  46.3: Action at 3.3 ('anon$0') for actor instance 'sec' might not preserve the channel invariant (#153)"} (forall i: int :: 
+    (0 <= i) && (i < (R[Net#b] + C[Net#b])) ==> (SqnCh[Net#b][i] == i)
+  );
+  assert {:msg "  47.3: Action at 3.3 ('anon$0') for actor instance 'sec' might not preserve the channel invariant (#154)"} (forall i: int :: 
+    (0 <= i) && (i < (R[Net#c] + C[Net#c])) ==> (SqnCh[Net#c][i] == i)
+  );
+  assert {:msg "  48.3: Action at 3.3 ('anon$0') for actor instance 'sec' might not preserve the channel invariant (#155)"} (forall i: int :: 
+    (0 <= i) && (i < (R[Net#d] + C[Net#d])) ==> (SqnCh[Net#d][i] == i)
+  );
+  assert {:msg "  49.3: Action at 3.3 ('anon$0') for actor instance 'sec' might not preserve the channel invariant (#156)"} (forall i: int :: 
+    (0 <= i) && (i < (R[Net#e] + C[Net#e])) ==> (SqnCh[Net#e][i] == i)
+  );
+  assert {:msg "  50.3: Action at 3.3 ('anon$0') for actor instance 'sec' might not preserve the channel invariant (#157)"} (forall i: int :: 
+    (0 <= i) && (i < (R[Net#g] + C[Net#g])) ==> (SqnCh[Net#g][i] == i)
+  );
+  assert {:msg "  52.3: Action at 3.3 ('anon$0') for actor instance 'sec' might not preserve the channel invariant (#158)"} C[Net#f] == 1;
+  assert {:msg "  53.3: Action at 3.3 ('anon$0') for actor instance 'sec' might not preserve the channel invariant (#159)"} C[Net#g] == R[Net#e];
+  assert {:msg "  54.3: Action at 3.3 ('anon$0') for actor instance 'sec' might not preserve the channel invariant (#160)"} R[Net#e] == M[Net#f][R[Net#f]];
+  assert {:msg "  55.3: Action at 3.3 ('anon$0') for actor instance 'sec' might not preserve the channel invariant (#161)"} (forall i: int :: 
+    (0 <= i) && (i < (R[Net#g] + C[Net#g])) ==> (SqnCh[Net#g][i] == i)
+  );
+  assert {:msg "  59.3: Action at 3.3 ('anon$0') for actor instance 'sec' might not preserve the channel invariant (#162)"} (0 < R[Net#d]) && (0 < R[Net#e]) ==> (M[Net#d][R[Net#d] - 1] <= M[Net#e][R[Net#e] - 1]);
+  assert {:msg "  60.3: Action at 3.3 ('anon$0') for actor instance 'sec' might not preserve the channel invariant (#163)"} (forall i: int :: 
     (0 <= i) && (i < R[Net#e]) ==> (M[Net#g][i] == M[Net#e][i])
   );
 }
-procedure Net#anon$2#Adjudicator#readoff#10()
+procedure Net#anon$3#Adjudicator#readoff#11()
   modifies C, R, M, St, SqnCh, SqnAct;
 {
-  var ActionPH#y1: int;
-  var ActionPH#y2: int;
-  var ActionPH#y3: int;
   var St#next: State;
   var x1#i: int;
   var c_in#c: int;
-  assume L[Net#a] == (3 * Base#L);
+  assume L[Net#a] == (1 * Base#L);
   assume 0 <= R[Net#a];
   assume 0 <= C[Net#a];
   assume (R[Net#a] + C[Net#a]) <= L[Net#a];
@@ -543,7 +695,6 @@ procedure Net#anon$2#Adjudicator#readoff#10()
   assume 0 <= R[Net#g];
   assume 0 <= C[Net#g];
   assume R[Net#g] == 0;
-  assume (M[Net#a][0] == 0) && (M[Net#a][1] == 1) && (M[Net#a][2] == 2);
   assume R[Net#a] == (R[Net#b] + C[Net#b]);
   assume R[Net#a] == (R[Net#c] + C[Net#c]);
   assume R[Net#b] == (R[Net#d] + C[Net#d]);
@@ -563,18 +714,41 @@ procedure Net#anon$2#Adjudicator#readoff#10()
   assume (forall idx$: int :: 
     (0 <= idx$) && (idx$ < (R[Net#a] + C[Net#a])) ==> (SqnCh[Net#a][idx$] == idx$)
   );
-  assume (R[Net#a] + C[Net#a]) <= 3;
+  assume SqnAct[Net#spl] == R[Net#a];
+  assume SqnAct[Net#pri] == R[Net#b];
+  assume SqnAct[Net#sec] == R[Net#c];
+  assume SqnAct[Net#adj] == R[Net#e];
+  assume (forall i: int :: 
+    (0 <= i) && (i < (R[Net#a] + C[Net#a])) ==> (SqnCh[Net#a][i] == i)
+  );
+  assume (forall i: int :: 
+    (0 <= i) && (i < (R[Net#b] + C[Net#b])) ==> (SqnCh[Net#b][i] == i)
+  );
+  assume (forall i: int :: 
+    (0 <= i) && (i < (R[Net#c] + C[Net#c])) ==> (SqnCh[Net#c][i] == i)
+  );
+  assume (forall i: int :: 
+    (0 <= i) && (i < (R[Net#d] + C[Net#d])) ==> (SqnCh[Net#d][i] == i)
+  );
+  assume (forall i: int :: 
+    (0 <= i) && (i < (R[Net#e] + C[Net#e])) ==> (SqnCh[Net#e][i] == i)
+  );
+  assume (forall i: int :: 
+    (0 <= i) && (i < (R[Net#g] + C[Net#g])) ==> (SqnCh[Net#g][i] == i)
+  );
   assume C[Net#f] == 1;
   assume C[Net#g] == R[Net#e];
   assume R[Net#e] == M[Net#f][R[Net#f]];
-  assume R[Net#d] <= R[Net#e];
+  assume (forall i: int :: 
+    (0 <= i) && (i < (R[Net#g] + C[Net#g])) ==> (SqnCh[Net#g][i] == i)
+  );
   assume (0 < R[Net#d]) && (0 < R[Net#e]) ==> (M[Net#d][R[Net#d] - 1] <= M[Net#e][R[Net#e] - 1]);
   assume (forall i: int :: 
     (0 <= i) && (i < R[Net#e]) ==> (M[Net#g][i] == M[Net#e][i])
   );
-  assume M[Net#d][R[Net#d] - 0] < M[Net#f][R[Net#f] - 0];
+  assume SqnCh[Net#d][R[Net#d] - 0] < M[Net#f][R[Net#f] - 0];
   assume true;
-  assume (1 <= C[Net#d]) && (1 <= C[Net#f]) && (M[Net#d][R[Net#d] - 0] < M[Net#f][R[Net#f] - 0]);
+  assume (1 <= C[Net#d]) && (1 <= C[Net#f]) && (SqnCh[Net#d][R[Net#d] - 0] < M[Net#f][R[Net#f] - 0]);
   x1#i := M[Net#d][R[Net#d]];
   R[Net#d] := R[Net#d] + 1;
   C[Net#d] := C[Net#d] - 1;
@@ -584,7 +758,6 @@ procedure Net#anon$2#Adjudicator#readoff#10()
   M[Net#f][R[Net#f] + C[Net#f]] := c_in#c;
   SqnCh[Net#f][R[Net#f] + C[Net#f]] := SqnAct[Net#adj];
   C[Net#f] := C[Net#f] + 1;
-  SqnAct[Net#adj] := SqnAct[Net#adj] + 1;
   assume 0 <= R[Net#a];
   assume 0 <= C[Net#a];
   assume (R[Net#a] + C[Net#a]) <= L[Net#a];
@@ -601,47 +774,66 @@ procedure Net#anon$2#Adjudicator#readoff#10()
   assume 0 <= R[Net#g];
   assume 0 <= C[Net#g];
   assume R[Net#g] == 0;
-  assert {:msg "  Action at 22.3 ('readoff') for actor instance 'adj' might not preserve the channel invariant (#148)"} (M[Net#a][0] == 0) && (M[Net#a][1] == 1) && (M[Net#a][2] == 2);
-  assert {:msg "  Action at 22.3 ('readoff') for actor instance 'adj' might not preserve the channel invariant (#149)"} R[Net#a] == (R[Net#b] + C[Net#b]);
-  assert {:msg "  Action at 22.3 ('readoff') for actor instance 'adj' might not preserve the channel invariant (#150)"} R[Net#a] == (R[Net#c] + C[Net#c]);
-  assert {:msg "  Action at 22.3 ('readoff') for actor instance 'adj' might not preserve the channel invariant (#151)"} R[Net#b] == (R[Net#d] + C[Net#d]);
-  assert {:msg "  Action at 22.3 ('readoff') for actor instance 'adj' might not preserve the channel invariant (#152)"} R[Net#c] == (R[Net#e] + C[Net#e]);
-  assert {:msg "  Action at 22.3 ('readoff') for actor instance 'adj' might not preserve the channel invariant (#153)"} (forall idx$: int :: 
+  assert {:msg "  Action at 20.3 ('readoff') for actor instance 'adj' might not preserve the channel invariant (#180)"} R[Net#a] == (R[Net#b] + C[Net#b]);
+  assert {:msg "  Action at 20.3 ('readoff') for actor instance 'adj' might not preserve the channel invariant (#181)"} R[Net#a] == (R[Net#c] + C[Net#c]);
+  assert {:msg "  Action at 20.3 ('readoff') for actor instance 'adj' might not preserve the channel invariant (#182)"} R[Net#b] == (R[Net#d] + C[Net#d]);
+  assert {:msg "  Action at 20.3 ('readoff') for actor instance 'adj' might not preserve the channel invariant (#183)"} R[Net#c] == (R[Net#e] + C[Net#e]);
+  assert {:msg "  Action at 20.3 ('readoff') for actor instance 'adj' might not preserve the channel invariant (#184)"} (forall idx$: int :: 
     (0 <= idx$) && (idx$ < (R[Net#b] + C[Net#b])) ==> (M[Net#b][idx$] == M[Net#a][idx$])
   );
-  assert {:msg "  Action at 22.3 ('readoff') for actor instance 'adj' might not preserve the channel invariant (#154)"} (forall idx$: int :: 
+  assert {:msg "  Action at 20.3 ('readoff') for actor instance 'adj' might not preserve the channel invariant (#185)"} (forall idx$: int :: 
     (0 <= idx$) && (idx$ < (R[Net#c] + C[Net#c])) ==> (M[Net#c][idx$] == M[Net#a][idx$])
   );
-  assert {:msg "  Action at 22.3 ('readoff') for actor instance 'adj' might not preserve the channel invariant (#155)"} (forall idx$: int :: 
+  assert {:msg "  Action at 20.3 ('readoff') for actor instance 'adj' might not preserve the channel invariant (#186)"} (forall idx$: int :: 
     (0 <= idx$) && (idx$ < (R[Net#d] + C[Net#d])) ==> (M[Net#d][idx$] == M[Net#b][idx$])
   );
-  assert {:msg "  Action at 22.3 ('readoff') for actor instance 'adj' might not preserve the channel invariant (#156)"} (forall idx$: int :: 
+  assert {:msg "  Action at 20.3 ('readoff') for actor instance 'adj' might not preserve the channel invariant (#187)"} (forall idx$: int :: 
     (0 <= idx$) && (idx$ < (R[Net#e] + C[Net#e])) ==> (M[Net#e][idx$] == M[Net#c][idx$])
   );
-  assert {:msg "  Action at 22.3 ('readoff') for actor instance 'adj' might not preserve the channel invariant (#157)"} (forall idx$: int :: 
+  assert {:msg "  Action at 20.3 ('readoff') for actor instance 'adj' might not preserve the channel invariant (#188)"} (forall idx$: int :: 
     (0 <= idx$) && (idx$ < (R[Net#a] + C[Net#a])) ==> (SqnCh[Net#a][idx$] == idx$)
   );
-  assert {:msg "  40.3: Action at 22.3 ('readoff') for actor instance 'adj' might not preserve the channel invariant (#158)"} (R[Net#a] + C[Net#a]) <= 3;
-  assert {:msg "  47.3: Action at 22.3 ('readoff') for actor instance 'adj' might not preserve the channel invariant (#159)"} C[Net#f] == 1;
-  assert {:msg "  48.3: Action at 22.3 ('readoff') for actor instance 'adj' might not preserve the channel invariant (#160)"} C[Net#g] == R[Net#e];
-  assert {:msg "  49.3: Action at 22.3 ('readoff') for actor instance 'adj' might not preserve the channel invariant (#161)"} R[Net#e] == M[Net#f][R[Net#f]];
-  assert {:msg "  50.3: Action at 22.3 ('readoff') for actor instance 'adj' might not preserve the channel invariant (#162)"} R[Net#d] <= R[Net#e];
-  assert {:msg "  51.3: Action at 22.3 ('readoff') for actor instance 'adj' might not preserve the channel invariant (#163)"} (0 < R[Net#d]) && (0 < R[Net#e]) ==> (M[Net#d][R[Net#d] - 1] <= M[Net#e][R[Net#e] - 1]);
-  assert {:msg "  52.3: Action at 22.3 ('readoff') for actor instance 'adj' might not preserve the channel invariant (#164)"} (forall i: int :: 
+  assert {:msg "  40.3: Action at 20.3 ('readoff') for actor instance 'adj' might not preserve the channel invariant (#189)"} SqnAct[Net#spl] == R[Net#a];
+  assert {:msg "  41.3: Action at 20.3 ('readoff') for actor instance 'adj' might not preserve the channel invariant (#190)"} SqnAct[Net#pri] == R[Net#b];
+  assert {:msg "  42.3: Action at 20.3 ('readoff') for actor instance 'adj' might not preserve the channel invariant (#191)"} SqnAct[Net#sec] == R[Net#c];
+  assert {:msg "  43.3: Action at 20.3 ('readoff') for actor instance 'adj' might not preserve the channel invariant (#192)"} SqnAct[Net#adj] == R[Net#e];
+  assert {:msg "  45.3: Action at 20.3 ('readoff') for actor instance 'adj' might not preserve the channel invariant (#193)"} (forall i: int :: 
+    (0 <= i) && (i < (R[Net#a] + C[Net#a])) ==> (SqnCh[Net#a][i] == i)
+  );
+  assert {:msg "  46.3: Action at 20.3 ('readoff') for actor instance 'adj' might not preserve the channel invariant (#194)"} (forall i: int :: 
+    (0 <= i) && (i < (R[Net#b] + C[Net#b])) ==> (SqnCh[Net#b][i] == i)
+  );
+  assert {:msg "  47.3: Action at 20.3 ('readoff') for actor instance 'adj' might not preserve the channel invariant (#195)"} (forall i: int :: 
+    (0 <= i) && (i < (R[Net#c] + C[Net#c])) ==> (SqnCh[Net#c][i] == i)
+  );
+  assert {:msg "  48.3: Action at 20.3 ('readoff') for actor instance 'adj' might not preserve the channel invariant (#196)"} (forall i: int :: 
+    (0 <= i) && (i < (R[Net#d] + C[Net#d])) ==> (SqnCh[Net#d][i] == i)
+  );
+  assert {:msg "  49.3: Action at 20.3 ('readoff') for actor instance 'adj' might not preserve the channel invariant (#197)"} (forall i: int :: 
+    (0 <= i) && (i < (R[Net#e] + C[Net#e])) ==> (SqnCh[Net#e][i] == i)
+  );
+  assert {:msg "  50.3: Action at 20.3 ('readoff') for actor instance 'adj' might not preserve the channel invariant (#198)"} (forall i: int :: 
+    (0 <= i) && (i < (R[Net#g] + C[Net#g])) ==> (SqnCh[Net#g][i] == i)
+  );
+  assert {:msg "  52.3: Action at 20.3 ('readoff') for actor instance 'adj' might not preserve the channel invariant (#199)"} C[Net#f] == 1;
+  assert {:msg "  53.3: Action at 20.3 ('readoff') for actor instance 'adj' might not preserve the channel invariant (#200)"} C[Net#g] == R[Net#e];
+  assert {:msg "  54.3: Action at 20.3 ('readoff') for actor instance 'adj' might not preserve the channel invariant (#201)"} R[Net#e] == M[Net#f][R[Net#f]];
+  assert {:msg "  55.3: Action at 20.3 ('readoff') for actor instance 'adj' might not preserve the channel invariant (#202)"} (forall i: int :: 
+    (0 <= i) && (i < (R[Net#g] + C[Net#g])) ==> (SqnCh[Net#g][i] == i)
+  );
+  assert {:msg "  59.3: Action at 20.3 ('readoff') for actor instance 'adj' might not preserve the channel invariant (#203)"} (0 < R[Net#d]) && (0 < R[Net#e]) ==> (M[Net#d][R[Net#d] - 1] <= M[Net#e][R[Net#e] - 1]);
+  assert {:msg "  60.3: Action at 20.3 ('readoff') for actor instance 'adj' might not preserve the channel invariant (#204)"} (forall i: int :: 
     (0 <= i) && (i < R[Net#e]) ==> (M[Net#g][i] == M[Net#e][i])
   );
 }
-procedure Net#anon$2#Adjudicator#normal#11()
+procedure Net#anon$3#Adjudicator#normal#12()
   modifies C, R, M, St, SqnCh, SqnAct;
 {
-  var ActionPH#y1: int;
-  var ActionPH#y2: int;
-  var ActionPH#y3: int;
   var St#next: State;
   var x1#i: int;
   var x2#j: int;
   var c_in#c: int;
-  assume L[Net#a] == (3 * Base#L);
+  assume L[Net#a] == (1 * Base#L);
   assume 0 <= R[Net#a];
   assume 0 <= C[Net#a];
   assume (R[Net#a] + C[Net#a]) <= L[Net#a];
@@ -658,7 +850,6 @@ procedure Net#anon$2#Adjudicator#normal#11()
   assume 0 <= R[Net#g];
   assume 0 <= C[Net#g];
   assume R[Net#g] == 0;
-  assume (M[Net#a][0] == 0) && (M[Net#a][1] == 1) && (M[Net#a][2] == 2);
   assume R[Net#a] == (R[Net#b] + C[Net#b]);
   assume R[Net#a] == (R[Net#c] + C[Net#c]);
   assume R[Net#b] == (R[Net#d] + C[Net#d]);
@@ -678,18 +869,41 @@ procedure Net#anon$2#Adjudicator#normal#11()
   assume (forall idx$: int :: 
     (0 <= idx$) && (idx$ < (R[Net#a] + C[Net#a])) ==> (SqnCh[Net#a][idx$] == idx$)
   );
-  assume (R[Net#a] + C[Net#a]) <= 3;
+  assume SqnAct[Net#spl] == R[Net#a];
+  assume SqnAct[Net#pri] == R[Net#b];
+  assume SqnAct[Net#sec] == R[Net#c];
+  assume SqnAct[Net#adj] == R[Net#e];
+  assume (forall i: int :: 
+    (0 <= i) && (i < (R[Net#a] + C[Net#a])) ==> (SqnCh[Net#a][i] == i)
+  );
+  assume (forall i: int :: 
+    (0 <= i) && (i < (R[Net#b] + C[Net#b])) ==> (SqnCh[Net#b][i] == i)
+  );
+  assume (forall i: int :: 
+    (0 <= i) && (i < (R[Net#c] + C[Net#c])) ==> (SqnCh[Net#c][i] == i)
+  );
+  assume (forall i: int :: 
+    (0 <= i) && (i < (R[Net#d] + C[Net#d])) ==> (SqnCh[Net#d][i] == i)
+  );
+  assume (forall i: int :: 
+    (0 <= i) && (i < (R[Net#e] + C[Net#e])) ==> (SqnCh[Net#e][i] == i)
+  );
+  assume (forall i: int :: 
+    (0 <= i) && (i < (R[Net#g] + C[Net#g])) ==> (SqnCh[Net#g][i] == i)
+  );
   assume C[Net#f] == 1;
   assume C[Net#g] == R[Net#e];
   assume R[Net#e] == M[Net#f][R[Net#f]];
-  assume R[Net#d] <= R[Net#e];
+  assume (forall i: int :: 
+    (0 <= i) && (i < (R[Net#g] + C[Net#g])) ==> (SqnCh[Net#g][i] == i)
+  );
   assume (0 < R[Net#d]) && (0 < R[Net#e]) ==> (M[Net#d][R[Net#d] - 1] <= M[Net#e][R[Net#e] - 1]);
   assume (forall i: int :: 
     (0 <= i) && (i < R[Net#e]) ==> (M[Net#g][i] == M[Net#e][i])
   );
-  assume (M[Net#d][R[Net#d] - 0] == M[Net#e][R[Net#e] - 0]) && (M[Net#d][R[Net#d] - 0] == M[Net#f][R[Net#f] - 0]);
+  assume (SqnCh[Net#d][R[Net#d] - 0] == SqnCh[Net#e][R[Net#e] - 0]) && (SqnCh[Net#d][R[Net#d] - 0] == M[Net#f][R[Net#f] - 0]);
   assume true;
-  assume (!((1 <= C[Net#d]) && (1 <= C[Net#f]) && (M[Net#d][R[Net#d] - 0] < M[Net#f][R[Net#f] - 0]))) && (1 <= C[Net#d]) && (1 <= C[Net#e]) && (1 <= C[Net#f]) && (M[Net#d][R[Net#d] - 0] == M[Net#e][R[Net#e] - 0]) && (M[Net#d][R[Net#d] - 0] == M[Net#f][R[Net#f] - 0]);
+  assume (!((1 <= C[Net#d]) && (1 <= C[Net#f]) && (SqnCh[Net#d][R[Net#d] - 0] < M[Net#f][R[Net#f] - 0]))) && (1 <= C[Net#d]) && (1 <= C[Net#e]) && (1 <= C[Net#f]) && (SqnCh[Net#d][R[Net#d] - 0] == SqnCh[Net#e][R[Net#e] - 0]) && (SqnCh[Net#d][R[Net#d] - 0] == M[Net#f][R[Net#f] - 0]);
   x1#i := M[Net#d][R[Net#d]];
   R[Net#d] := R[Net#d] + 1;
   C[Net#d] := C[Net#d] - 1;
@@ -722,46 +936,65 @@ procedure Net#anon$2#Adjudicator#normal#11()
   assume 0 <= R[Net#g];
   assume 0 <= C[Net#g];
   assume R[Net#g] == 0;
-  assert {:msg "  Action at 14.3 ('normal') for actor instance 'adj' might not preserve the channel invariant (#181)"} (M[Net#a][0] == 0) && (M[Net#a][1] == 1) && (M[Net#a][2] == 2);
-  assert {:msg "  Action at 14.3 ('normal') for actor instance 'adj' might not preserve the channel invariant (#182)"} R[Net#a] == (R[Net#b] + C[Net#b]);
-  assert {:msg "  Action at 14.3 ('normal') for actor instance 'adj' might not preserve the channel invariant (#183)"} R[Net#a] == (R[Net#c] + C[Net#c]);
-  assert {:msg "  Action at 14.3 ('normal') for actor instance 'adj' might not preserve the channel invariant (#184)"} R[Net#b] == (R[Net#d] + C[Net#d]);
-  assert {:msg "  Action at 14.3 ('normal') for actor instance 'adj' might not preserve the channel invariant (#185)"} R[Net#c] == (R[Net#e] + C[Net#e]);
-  assert {:msg "  Action at 14.3 ('normal') for actor instance 'adj' might not preserve the channel invariant (#186)"} (forall idx$: int :: 
+  assert {:msg "  Action at 14.3 ('normal') for actor instance 'adj' might not preserve the channel invariant (#221)"} R[Net#a] == (R[Net#b] + C[Net#b]);
+  assert {:msg "  Action at 14.3 ('normal') for actor instance 'adj' might not preserve the channel invariant (#222)"} R[Net#a] == (R[Net#c] + C[Net#c]);
+  assert {:msg "  Action at 14.3 ('normal') for actor instance 'adj' might not preserve the channel invariant (#223)"} R[Net#b] == (R[Net#d] + C[Net#d]);
+  assert {:msg "  Action at 14.3 ('normal') for actor instance 'adj' might not preserve the channel invariant (#224)"} R[Net#c] == (R[Net#e] + C[Net#e]);
+  assert {:msg "  Action at 14.3 ('normal') for actor instance 'adj' might not preserve the channel invariant (#225)"} (forall idx$: int :: 
     (0 <= idx$) && (idx$ < (R[Net#b] + C[Net#b])) ==> (M[Net#b][idx$] == M[Net#a][idx$])
   );
-  assert {:msg "  Action at 14.3 ('normal') for actor instance 'adj' might not preserve the channel invariant (#187)"} (forall idx$: int :: 
+  assert {:msg "  Action at 14.3 ('normal') for actor instance 'adj' might not preserve the channel invariant (#226)"} (forall idx$: int :: 
     (0 <= idx$) && (idx$ < (R[Net#c] + C[Net#c])) ==> (M[Net#c][idx$] == M[Net#a][idx$])
   );
-  assert {:msg "  Action at 14.3 ('normal') for actor instance 'adj' might not preserve the channel invariant (#188)"} (forall idx$: int :: 
+  assert {:msg "  Action at 14.3 ('normal') for actor instance 'adj' might not preserve the channel invariant (#227)"} (forall idx$: int :: 
     (0 <= idx$) && (idx$ < (R[Net#d] + C[Net#d])) ==> (M[Net#d][idx$] == M[Net#b][idx$])
   );
-  assert {:msg "  Action at 14.3 ('normal') for actor instance 'adj' might not preserve the channel invariant (#189)"} (forall idx$: int :: 
+  assert {:msg "  Action at 14.3 ('normal') for actor instance 'adj' might not preserve the channel invariant (#228)"} (forall idx$: int :: 
     (0 <= idx$) && (idx$ < (R[Net#e] + C[Net#e])) ==> (M[Net#e][idx$] == M[Net#c][idx$])
   );
-  assert {:msg "  Action at 14.3 ('normal') for actor instance 'adj' might not preserve the channel invariant (#190)"} (forall idx$: int :: 
+  assert {:msg "  Action at 14.3 ('normal') for actor instance 'adj' might not preserve the channel invariant (#229)"} (forall idx$: int :: 
     (0 <= idx$) && (idx$ < (R[Net#a] + C[Net#a])) ==> (SqnCh[Net#a][idx$] == idx$)
   );
-  assert {:msg "  40.3: Action at 14.3 ('normal') for actor instance 'adj' might not preserve the channel invariant (#191)"} (R[Net#a] + C[Net#a]) <= 3;
-  assert {:msg "  47.3: Action at 14.3 ('normal') for actor instance 'adj' might not preserve the channel invariant (#192)"} C[Net#f] == 1;
-  assert {:msg "  48.3: Action at 14.3 ('normal') for actor instance 'adj' might not preserve the channel invariant (#193)"} C[Net#g] == R[Net#e];
-  assert {:msg "  49.3: Action at 14.3 ('normal') for actor instance 'adj' might not preserve the channel invariant (#194)"} R[Net#e] == M[Net#f][R[Net#f]];
-  assert {:msg "  50.3: Action at 14.3 ('normal') for actor instance 'adj' might not preserve the channel invariant (#195)"} R[Net#d] <= R[Net#e];
-  assert {:msg "  51.3: Action at 14.3 ('normal') for actor instance 'adj' might not preserve the channel invariant (#196)"} (0 < R[Net#d]) && (0 < R[Net#e]) ==> (M[Net#d][R[Net#d] - 1] <= M[Net#e][R[Net#e] - 1]);
-  assert {:msg "  52.3: Action at 14.3 ('normal') for actor instance 'adj' might not preserve the channel invariant (#197)"} (forall i: int :: 
+  assert {:msg "  40.3: Action at 14.3 ('normal') for actor instance 'adj' might not preserve the channel invariant (#230)"} SqnAct[Net#spl] == R[Net#a];
+  assert {:msg "  41.3: Action at 14.3 ('normal') for actor instance 'adj' might not preserve the channel invariant (#231)"} SqnAct[Net#pri] == R[Net#b];
+  assert {:msg "  42.3: Action at 14.3 ('normal') for actor instance 'adj' might not preserve the channel invariant (#232)"} SqnAct[Net#sec] == R[Net#c];
+  assert {:msg "  43.3: Action at 14.3 ('normal') for actor instance 'adj' might not preserve the channel invariant (#233)"} SqnAct[Net#adj] == R[Net#e];
+  assert {:msg "  45.3: Action at 14.3 ('normal') for actor instance 'adj' might not preserve the channel invariant (#234)"} (forall i: int :: 
+    (0 <= i) && (i < (R[Net#a] + C[Net#a])) ==> (SqnCh[Net#a][i] == i)
+  );
+  assert {:msg "  46.3: Action at 14.3 ('normal') for actor instance 'adj' might not preserve the channel invariant (#235)"} (forall i: int :: 
+    (0 <= i) && (i < (R[Net#b] + C[Net#b])) ==> (SqnCh[Net#b][i] == i)
+  );
+  assert {:msg "  47.3: Action at 14.3 ('normal') for actor instance 'adj' might not preserve the channel invariant (#236)"} (forall i: int :: 
+    (0 <= i) && (i < (R[Net#c] + C[Net#c])) ==> (SqnCh[Net#c][i] == i)
+  );
+  assert {:msg "  48.3: Action at 14.3 ('normal') for actor instance 'adj' might not preserve the channel invariant (#237)"} (forall i: int :: 
+    (0 <= i) && (i < (R[Net#d] + C[Net#d])) ==> (SqnCh[Net#d][i] == i)
+  );
+  assert {:msg "  49.3: Action at 14.3 ('normal') for actor instance 'adj' might not preserve the channel invariant (#238)"} (forall i: int :: 
+    (0 <= i) && (i < (R[Net#e] + C[Net#e])) ==> (SqnCh[Net#e][i] == i)
+  );
+  assert {:msg "  50.3: Action at 14.3 ('normal') for actor instance 'adj' might not preserve the channel invariant (#239)"} (forall i: int :: 
+    (0 <= i) && (i < (R[Net#g] + C[Net#g])) ==> (SqnCh[Net#g][i] == i)
+  );
+  assert {:msg "  52.3: Action at 14.3 ('normal') for actor instance 'adj' might not preserve the channel invariant (#240)"} C[Net#f] == 1;
+  assert {:msg "  53.3: Action at 14.3 ('normal') for actor instance 'adj' might not preserve the channel invariant (#241)"} C[Net#g] == R[Net#e];
+  assert {:msg "  54.3: Action at 14.3 ('normal') for actor instance 'adj' might not preserve the channel invariant (#242)"} R[Net#e] == M[Net#f][R[Net#f]];
+  assert {:msg "  55.3: Action at 14.3 ('normal') for actor instance 'adj' might not preserve the channel invariant (#243)"} (forall i: int :: 
+    (0 <= i) && (i < (R[Net#g] + C[Net#g])) ==> (SqnCh[Net#g][i] == i)
+  );
+  assert {:msg "  59.3: Action at 14.3 ('normal') for actor instance 'adj' might not preserve the channel invariant (#244)"} (0 < R[Net#d]) && (0 < R[Net#e]) ==> (M[Net#d][R[Net#d] - 1] <= M[Net#e][R[Net#e] - 1]);
+  assert {:msg "  60.3: Action at 14.3 ('normal') for actor instance 'adj' might not preserve the channel invariant (#245)"} (forall i: int :: 
     (0 <= i) && (i < R[Net#e]) ==> (M[Net#g][i] == M[Net#e][i])
   );
 }
-procedure Net#anon$2#Adjudicator#timeout#12()
+procedure Net#anon$3#Adjudicator#timeout#13()
   modifies C, R, M, St, SqnCh, SqnAct;
 {
-  var ActionPH#y1: int;
-  var ActionPH#y2: int;
-  var ActionPH#y3: int;
   var St#next: State;
   var x2#j: int;
   var c_in#c: int;
-  assume L[Net#a] == (3 * Base#L);
+  assume L[Net#a] == (1 * Base#L);
   assume 0 <= R[Net#a];
   assume 0 <= C[Net#a];
   assume (R[Net#a] + C[Net#a]) <= L[Net#a];
@@ -778,7 +1011,6 @@ procedure Net#anon$2#Adjudicator#timeout#12()
   assume 0 <= R[Net#g];
   assume 0 <= C[Net#g];
   assume R[Net#g] == 0;
-  assume (M[Net#a][0] == 0) && (M[Net#a][1] == 1) && (M[Net#a][2] == 2);
   assume R[Net#a] == (R[Net#b] + C[Net#b]);
   assume R[Net#a] == (R[Net#c] + C[Net#c]);
   assume R[Net#b] == (R[Net#d] + C[Net#d]);
@@ -798,17 +1030,40 @@ procedure Net#anon$2#Adjudicator#timeout#12()
   assume (forall idx$: int :: 
     (0 <= idx$) && (idx$ < (R[Net#a] + C[Net#a])) ==> (SqnCh[Net#a][idx$] == idx$)
   );
-  assume (R[Net#a] + C[Net#a]) <= 3;
+  assume SqnAct[Net#spl] == R[Net#a];
+  assume SqnAct[Net#pri] == R[Net#b];
+  assume SqnAct[Net#sec] == R[Net#c];
+  assume SqnAct[Net#adj] == R[Net#e];
+  assume (forall i: int :: 
+    (0 <= i) && (i < (R[Net#a] + C[Net#a])) ==> (SqnCh[Net#a][i] == i)
+  );
+  assume (forall i: int :: 
+    (0 <= i) && (i < (R[Net#b] + C[Net#b])) ==> (SqnCh[Net#b][i] == i)
+  );
+  assume (forall i: int :: 
+    (0 <= i) && (i < (R[Net#c] + C[Net#c])) ==> (SqnCh[Net#c][i] == i)
+  );
+  assume (forall i: int :: 
+    (0 <= i) && (i < (R[Net#d] + C[Net#d])) ==> (SqnCh[Net#d][i] == i)
+  );
+  assume (forall i: int :: 
+    (0 <= i) && (i < (R[Net#e] + C[Net#e])) ==> (SqnCh[Net#e][i] == i)
+  );
+  assume (forall i: int :: 
+    (0 <= i) && (i < (R[Net#g] + C[Net#g])) ==> (SqnCh[Net#g][i] == i)
+  );
   assume C[Net#f] == 1;
   assume C[Net#g] == R[Net#e];
   assume R[Net#e] == M[Net#f][R[Net#f]];
-  assume R[Net#d] <= R[Net#e];
+  assume (forall i: int :: 
+    (0 <= i) && (i < (R[Net#g] + C[Net#g])) ==> (SqnCh[Net#g][i] == i)
+  );
   assume (0 < R[Net#d]) && (0 < R[Net#e]) ==> (M[Net#d][R[Net#d] - 1] <= M[Net#e][R[Net#e] - 1]);
   assume (forall i: int :: 
     (0 <= i) && (i < R[Net#e]) ==> (M[Net#g][i] == M[Net#e][i])
   );
   assume true;
-  assume (!((1 <= C[Net#d]) && (1 <= C[Net#f]) && (M[Net#d][R[Net#d] - 0] < M[Net#f][R[Net#f] - 0]))) && (!((1 <= C[Net#d]) && (1 <= C[Net#e]) && (1 <= C[Net#f]) && (M[Net#d][R[Net#d] - 0] == M[Net#e][R[Net#e] - 0]) && (M[Net#d][R[Net#d] - 0] == M[Net#f][R[Net#f] - 0]))) && (1 <= C[Net#e]) && (1 <= C[Net#f]);
+  assume (!((1 <= C[Net#d]) && (1 <= C[Net#f]) && (SqnCh[Net#d][R[Net#d] - 0] < M[Net#f][R[Net#f] - 0]))) && (!((1 <= C[Net#d]) && (1 <= C[Net#e]) && (1 <= C[Net#f]) && (SqnCh[Net#d][R[Net#d] - 0] == SqnCh[Net#e][R[Net#e] - 0]) && (SqnCh[Net#d][R[Net#d] - 0] == M[Net#f][R[Net#f] - 0]))) && (1 <= C[Net#e]) && (1 <= C[Net#f]);
   x2#j := M[Net#e][R[Net#e]];
   R[Net#e] := R[Net#e] + 1;
   C[Net#e] := C[Net#e] - 1;
@@ -838,43 +1093,62 @@ procedure Net#anon$2#Adjudicator#timeout#12()
   assume 0 <= R[Net#g];
   assume 0 <= C[Net#g];
   assume R[Net#g] == 0;
-  assert {:msg "  Action at 18.3 ('timeout') for actor instance 'adj' might not preserve the channel invariant (#214)"} (M[Net#a][0] == 0) && (M[Net#a][1] == 1) && (M[Net#a][2] == 2);
-  assert {:msg "  Action at 18.3 ('timeout') for actor instance 'adj' might not preserve the channel invariant (#215)"} R[Net#a] == (R[Net#b] + C[Net#b]);
-  assert {:msg "  Action at 18.3 ('timeout') for actor instance 'adj' might not preserve the channel invariant (#216)"} R[Net#a] == (R[Net#c] + C[Net#c]);
-  assert {:msg "  Action at 18.3 ('timeout') for actor instance 'adj' might not preserve the channel invariant (#217)"} R[Net#b] == (R[Net#d] + C[Net#d]);
-  assert {:msg "  Action at 18.3 ('timeout') for actor instance 'adj' might not preserve the channel invariant (#218)"} R[Net#c] == (R[Net#e] + C[Net#e]);
-  assert {:msg "  Action at 18.3 ('timeout') for actor instance 'adj' might not preserve the channel invariant (#219)"} (forall idx$: int :: 
+  assert {:msg "  Action at 18.3 ('timeout') for actor instance 'adj' might not preserve the channel invariant (#262)"} R[Net#a] == (R[Net#b] + C[Net#b]);
+  assert {:msg "  Action at 18.3 ('timeout') for actor instance 'adj' might not preserve the channel invariant (#263)"} R[Net#a] == (R[Net#c] + C[Net#c]);
+  assert {:msg "  Action at 18.3 ('timeout') for actor instance 'adj' might not preserve the channel invariant (#264)"} R[Net#b] == (R[Net#d] + C[Net#d]);
+  assert {:msg "  Action at 18.3 ('timeout') for actor instance 'adj' might not preserve the channel invariant (#265)"} R[Net#c] == (R[Net#e] + C[Net#e]);
+  assert {:msg "  Action at 18.3 ('timeout') for actor instance 'adj' might not preserve the channel invariant (#266)"} (forall idx$: int :: 
     (0 <= idx$) && (idx$ < (R[Net#b] + C[Net#b])) ==> (M[Net#b][idx$] == M[Net#a][idx$])
   );
-  assert {:msg "  Action at 18.3 ('timeout') for actor instance 'adj' might not preserve the channel invariant (#220)"} (forall idx$: int :: 
+  assert {:msg "  Action at 18.3 ('timeout') for actor instance 'adj' might not preserve the channel invariant (#267)"} (forall idx$: int :: 
     (0 <= idx$) && (idx$ < (R[Net#c] + C[Net#c])) ==> (M[Net#c][idx$] == M[Net#a][idx$])
   );
-  assert {:msg "  Action at 18.3 ('timeout') for actor instance 'adj' might not preserve the channel invariant (#221)"} (forall idx$: int :: 
+  assert {:msg "  Action at 18.3 ('timeout') for actor instance 'adj' might not preserve the channel invariant (#268)"} (forall idx$: int :: 
     (0 <= idx$) && (idx$ < (R[Net#d] + C[Net#d])) ==> (M[Net#d][idx$] == M[Net#b][idx$])
   );
-  assert {:msg "  Action at 18.3 ('timeout') for actor instance 'adj' might not preserve the channel invariant (#222)"} (forall idx$: int :: 
+  assert {:msg "  Action at 18.3 ('timeout') for actor instance 'adj' might not preserve the channel invariant (#269)"} (forall idx$: int :: 
     (0 <= idx$) && (idx$ < (R[Net#e] + C[Net#e])) ==> (M[Net#e][idx$] == M[Net#c][idx$])
   );
-  assert {:msg "  Action at 18.3 ('timeout') for actor instance 'adj' might not preserve the channel invariant (#223)"} (forall idx$: int :: 
+  assert {:msg "  Action at 18.3 ('timeout') for actor instance 'adj' might not preserve the channel invariant (#270)"} (forall idx$: int :: 
     (0 <= idx$) && (idx$ < (R[Net#a] + C[Net#a])) ==> (SqnCh[Net#a][idx$] == idx$)
   );
-  assert {:msg "  40.3: Action at 18.3 ('timeout') for actor instance 'adj' might not preserve the channel invariant (#224)"} (R[Net#a] + C[Net#a]) <= 3;
-  assert {:msg "  47.3: Action at 18.3 ('timeout') for actor instance 'adj' might not preserve the channel invariant (#225)"} C[Net#f] == 1;
-  assert {:msg "  48.3: Action at 18.3 ('timeout') for actor instance 'adj' might not preserve the channel invariant (#226)"} C[Net#g] == R[Net#e];
-  assert {:msg "  49.3: Action at 18.3 ('timeout') for actor instance 'adj' might not preserve the channel invariant (#227)"} R[Net#e] == M[Net#f][R[Net#f]];
-  assert {:msg "  50.3: Action at 18.3 ('timeout') for actor instance 'adj' might not preserve the channel invariant (#228)"} R[Net#d] <= R[Net#e];
-  assert {:msg "  51.3: Action at 18.3 ('timeout') for actor instance 'adj' might not preserve the channel invariant (#229)"} (0 < R[Net#d]) && (0 < R[Net#e]) ==> (M[Net#d][R[Net#d] - 1] <= M[Net#e][R[Net#e] - 1]);
-  assert {:msg "  52.3: Action at 18.3 ('timeout') for actor instance 'adj' might not preserve the channel invariant (#230)"} (forall i: int :: 
+  assert {:msg "  40.3: Action at 18.3 ('timeout') for actor instance 'adj' might not preserve the channel invariant (#271)"} SqnAct[Net#spl] == R[Net#a];
+  assert {:msg "  41.3: Action at 18.3 ('timeout') for actor instance 'adj' might not preserve the channel invariant (#272)"} SqnAct[Net#pri] == R[Net#b];
+  assert {:msg "  42.3: Action at 18.3 ('timeout') for actor instance 'adj' might not preserve the channel invariant (#273)"} SqnAct[Net#sec] == R[Net#c];
+  assert {:msg "  43.3: Action at 18.3 ('timeout') for actor instance 'adj' might not preserve the channel invariant (#274)"} SqnAct[Net#adj] == R[Net#e];
+  assert {:msg "  45.3: Action at 18.3 ('timeout') for actor instance 'adj' might not preserve the channel invariant (#275)"} (forall i: int :: 
+    (0 <= i) && (i < (R[Net#a] + C[Net#a])) ==> (SqnCh[Net#a][i] == i)
+  );
+  assert {:msg "  46.3: Action at 18.3 ('timeout') for actor instance 'adj' might not preserve the channel invariant (#276)"} (forall i: int :: 
+    (0 <= i) && (i < (R[Net#b] + C[Net#b])) ==> (SqnCh[Net#b][i] == i)
+  );
+  assert {:msg "  47.3: Action at 18.3 ('timeout') for actor instance 'adj' might not preserve the channel invariant (#277)"} (forall i: int :: 
+    (0 <= i) && (i < (R[Net#c] + C[Net#c])) ==> (SqnCh[Net#c][i] == i)
+  );
+  assert {:msg "  48.3: Action at 18.3 ('timeout') for actor instance 'adj' might not preserve the channel invariant (#278)"} (forall i: int :: 
+    (0 <= i) && (i < (R[Net#d] + C[Net#d])) ==> (SqnCh[Net#d][i] == i)
+  );
+  assert {:msg "  49.3: Action at 18.3 ('timeout') for actor instance 'adj' might not preserve the channel invariant (#279)"} (forall i: int :: 
+    (0 <= i) && (i < (R[Net#e] + C[Net#e])) ==> (SqnCh[Net#e][i] == i)
+  );
+  assert {:msg "  50.3: Action at 18.3 ('timeout') for actor instance 'adj' might not preserve the channel invariant (#280)"} (forall i: int :: 
+    (0 <= i) && (i < (R[Net#g] + C[Net#g])) ==> (SqnCh[Net#g][i] == i)
+  );
+  assert {:msg "  52.3: Action at 18.3 ('timeout') for actor instance 'adj' might not preserve the channel invariant (#281)"} C[Net#f] == 1;
+  assert {:msg "  53.3: Action at 18.3 ('timeout') for actor instance 'adj' might not preserve the channel invariant (#282)"} C[Net#g] == R[Net#e];
+  assert {:msg "  54.3: Action at 18.3 ('timeout') for actor instance 'adj' might not preserve the channel invariant (#283)"} R[Net#e] == M[Net#f][R[Net#f]];
+  assert {:msg "  55.3: Action at 18.3 ('timeout') for actor instance 'adj' might not preserve the channel invariant (#284)"} (forall i: int :: 
+    (0 <= i) && (i < (R[Net#g] + C[Net#g])) ==> (SqnCh[Net#g][i] == i)
+  );
+  assert {:msg "  59.3: Action at 18.3 ('timeout') for actor instance 'adj' might not preserve the channel invariant (#285)"} (0 < R[Net#d]) && (0 < R[Net#e]) ==> (M[Net#d][R[Net#d] - 1] <= M[Net#e][R[Net#e] - 1]);
+  assert {:msg "  60.3: Action at 18.3 ('timeout') for actor instance 'adj' might not preserve the channel invariant (#286)"} (forall i: int :: 
     (0 <= i) && (i < R[Net#e]) ==> (M[Net#g][i] == M[Net#e][i])
   );
 }
-procedure Net#anon$2#exit#13()
+procedure Net#anon$3#exit#14()
   modifies C, R, M, St, SqnCh, SqnAct;
 {
-  var ActionPH#y1: int;
-  var ActionPH#y2: int;
-  var ActionPH#y3: int;
-  assume L[Net#a] == (3 * Base#L);
+  assume L[Net#a] == (1 * Base#L);
   assume 0 <= R[Net#a];
   assume 0 <= C[Net#a];
   assume (R[Net#a] + C[Net#a]) <= L[Net#a];
@@ -891,7 +1165,6 @@ procedure Net#anon$2#exit#13()
   assume 0 <= R[Net#g];
   assume 0 <= C[Net#g];
   assume R[Net#g] == 0;
-  assume (M[Net#a][0] == 0) && (M[Net#a][1] == 1) && (M[Net#a][2] == 2);
   assume R[Net#a] == (R[Net#b] + C[Net#b]);
   assume R[Net#a] == (R[Net#c] + C[Net#c]);
   assume R[Net#b] == (R[Net#d] + C[Net#d]);
@@ -911,11 +1184,34 @@ procedure Net#anon$2#exit#13()
   assume (forall idx$: int :: 
     (0 <= idx$) && (idx$ < (R[Net#a] + C[Net#a])) ==> (SqnCh[Net#a][idx$] == idx$)
   );
-  assume (R[Net#a] + C[Net#a]) <= 3;
+  assume SqnAct[Net#spl] == R[Net#a];
+  assume SqnAct[Net#pri] == R[Net#b];
+  assume SqnAct[Net#sec] == R[Net#c];
+  assume SqnAct[Net#adj] == R[Net#e];
+  assume (forall i: int :: 
+    (0 <= i) && (i < (R[Net#a] + C[Net#a])) ==> (SqnCh[Net#a][i] == i)
+  );
+  assume (forall i: int :: 
+    (0 <= i) && (i < (R[Net#b] + C[Net#b])) ==> (SqnCh[Net#b][i] == i)
+  );
+  assume (forall i: int :: 
+    (0 <= i) && (i < (R[Net#c] + C[Net#c])) ==> (SqnCh[Net#c][i] == i)
+  );
+  assume (forall i: int :: 
+    (0 <= i) && (i < (R[Net#d] + C[Net#d])) ==> (SqnCh[Net#d][i] == i)
+  );
+  assume (forall i: int :: 
+    (0 <= i) && (i < (R[Net#e] + C[Net#e])) ==> (SqnCh[Net#e][i] == i)
+  );
+  assume (forall i: int :: 
+    (0 <= i) && (i < (R[Net#g] + C[Net#g])) ==> (SqnCh[Net#g][i] == i)
+  );
   assume C[Net#f] == 1;
   assume C[Net#g] == R[Net#e];
   assume R[Net#e] == M[Net#f][R[Net#f]];
-  assume R[Net#d] <= R[Net#e];
+  assume (forall i: int :: 
+    (0 <= i) && (i < (R[Net#g] + C[Net#g])) ==> (SqnCh[Net#g][i] == i)
+  );
   assume (0 < R[Net#d]) && (0 < R[Net#e]) ==> (M[Net#d][R[Net#d] - 1] <= M[Net#e][R[Net#e] - 1]);
   assume (forall i: int :: 
     (0 <= i) && (i < R[Net#e]) ==> (M[Net#g][i] == M[Net#e][i])
@@ -924,17 +1220,19 @@ procedure Net#anon$2#exit#13()
   assume !(1 <= C[Net#a]);
   assume !(1 <= C[Net#b]);
   assume !(1 <= C[Net#c]);
-  assume !((!((1 <= C[Net#d]) && (1 <= C[Net#f]) && (M[Net#d][R[Net#d] - 0] < M[Net#f][R[Net#f] - 0]))) && (1 <= C[Net#d]) && (1 <= C[Net#e]) && (1 <= C[Net#f]) && (M[Net#d][R[Net#d] - 0] == M[Net#e][R[Net#e] - 0]) && (M[Net#d][R[Net#d] - 0] == M[Net#f][R[Net#f] - 0]));
-  assume !((1 <= C[Net#d]) && (1 <= C[Net#f]) && (M[Net#d][R[Net#d] - 0] < M[Net#f][R[Net#f] - 0]));
-  assume !((!((1 <= C[Net#d]) && (1 <= C[Net#f]) && (M[Net#d][R[Net#d] - 0] < M[Net#f][R[Net#f] - 0]))) && (!((1 <= C[Net#d]) && (1 <= C[Net#e]) && (1 <= C[Net#f]) && (M[Net#d][R[Net#d] - 0] == M[Net#e][R[Net#e] - 0]) && (M[Net#d][R[Net#d] - 0] == M[Net#f][R[Net#f] - 0]))) && (1 <= C[Net#e]) && (1 <= C[Net#f]));
-  ActionPH#y1 := M[Net#g][0];
-  ActionPH#y2 := M[Net#g][1];
-  ActionPH#y3 := M[Net#g][2];
-  assert {:msg "  34.13: Network action postcondition might not hold"} (ActionPH#y1 == M[Net#a][0]) && (ActionPH#y2 == M[Net#a][1]) && (ActionPH#y3 == M[Net#a][2]);
+  assume !((!((1 <= C[Net#d]) && (1 <= C[Net#f]) && (SqnCh[Net#d][R[Net#d] - 0] < M[Net#f][R[Net#f] - 0]))) && (1 <= C[Net#d]) && (1 <= C[Net#e]) && (1 <= C[Net#f]) && (SqnCh[Net#d][R[Net#d] - 0] == SqnCh[Net#e][R[Net#e] - 0]) && (SqnCh[Net#d][R[Net#d] - 0] == M[Net#f][R[Net#f] - 0]));
+  assume !((!((1 <= C[Net#d]) && (1 <= C[Net#f]) && (SqnCh[Net#d][R[Net#d] - 0] < M[Net#f][R[Net#f] - 0]))) && (!((1 <= C[Net#d]) && (1 <= C[Net#e]) && (1 <= C[Net#f]) && (SqnCh[Net#d][R[Net#d] - 0] == SqnCh[Net#e][R[Net#e] - 0]) && (SqnCh[Net#d][R[Net#d] - 0] == M[Net#f][R[Net#f] - 0]))) && (1 <= C[Net#e]) && (1 <= C[Net#f]));
+  assume !((1 <= C[Net#d]) && (1 <= C[Net#f]) && (SqnCh[Net#d][R[Net#d] - 0] < M[Net#f][R[Net#f] - 0]));
+  assert {:msg "  33.14: Network action postcondition might not hold"} (forall i: int :: 
+    (0 <= i) && (i < (R[Net#g] + C[Net#g])) ==> (SqnCh[Net#g][i] == i)
+  );
+  assert {:msg "  34.14: Network action postcondition might not hold"} (forall i: int :: 
+    (0 <= i) && (i < (R[Net#g] + C[Net#g])) ==> (M[Net#g][i] == M[Net#a][i])
+  );
   R[Net#g] := R[Net#g] + C[Net#g];
-  C[Net#g] := C[Net#g] - (3 * Base#L);
+  C[Net#g] := C[Net#g] - (1 * Base#L);
   C[Net#f] := C[Net#f] - 1;
-  assume M[Net#f][R[Net#f]] == 0;
+  assert {:msg "  38.13: The network might not preserve the network invariant"} R[Net#e] == M[Net#f][R[Net#f]];
   assert {:msg "  32.3: The network might leave unread tokens on channel a"} C[Net#a] == 0;
   assert {:msg "  32.3: The network might leave unread tokens on channel b"} C[Net#b] == 0;
   assert {:msg "  32.3: The network might leave unread tokens on channel c"} C[Net#c] == 0;
